theories/rules/rules_IsUnique.v
@@ -20,67 +20,6 @@ Section cap_lang_rules.
   Implicit Types mem : Mem.
   Implicit Types lmem : LMem.
 
-  (* TODO is this definition convenient enough ?
-     The details does not really matter, as soon as the following lemma
-     is proven. *)
-  (* TODO move somewhere ? *)
-  Definition update_version_word_region (lmem : LMem) (lwsrc : LWord)
-    : option LMem :=
-    match lwsrc with
-    | LCap _ b e _ v
-    | LSealedCap _ _ b e _ v =>
-        foldr
-          ( fun a upd_opt => lmem' ← upd_opt; update_version_addr lmem' a v)
-          (Some lmem)
-          (finz.seq_between b e)
-    | _ => Some lmem
-    end.
-
-  Lemma update_cur_version_region_implies_next_version_gen
-    (lm lm' : LMem) (cur_map cur_map': VMap) (la : list Addr) (v : Version) :
-    NoDup la ->
-    (∀ a : Addr, a ∈ la → cur_map !! a = Some v) ->
-    update_cur_version_region lm cur_map la = Some (lm', cur_map') ->
-    foldr
-      (λ (a0 : Addr) (upd_opt : option LMem),
-        upd_opt ≫= (λ lmem', update_version_addr lmem' a0 v))
-      (Some lm) la = Some lm'.
-  Proof.
-    move: lm lm' cur_map cur_map' v.
-    induction la as [|a la Hla]; intros * HNoDup Hcur_addr Hupd.
-    - by cbn in *; simplify_eq.
-    - cbn in *.
-      apply NoDup_cons in HNoDup ; destruct HNoDup as [Ha_notin_la HNoDup].
-      assert (Hcur_a : cur_map !! a = Some v).
-      { apply Hcur_addr, elem_of_cons; by left. }
-      assert (Hcur_addr' : ∀ a0 : Addr, a0 ∈ la → cur_map !! a0 = Some v).
-      { intros a' Hin. apply Hcur_addr, elem_of_cons; by right. }
-      rewrite -/(update_cur_version_region lm cur_map la) in Hupd.
-      apply bind_Some in Hupd.
-      destruct Hupd as ( [lmem0 cur_map0] & Hupd & Hupd0 ).
-      erewrite Hla ; eauto.
-      cbn.
-      opose proof (
-          update_cur_version_region_notin_preserves_cur_map
-            lm lmem0 cur_map cur_map0 la a v _ _ _)
-        as Hcur0_a; eauto.
-      rewrite /update_cur_version_addr Hcur0_a /= in Hupd0.
-      apply bind_Some in Hupd0.
-      by destruct Hupd0 as (lm0 & Hlm0 & ?) ; simplify_eq.
-  Qed.
-
-  Lemma update_cur_version_region_implies_next_version
-    (lm lm' : LMem) (cur_map cur_map': VMap)
-    (p : Perm) (b e a : Addr) (v : Version) :
-    is_cur_word (LCap p b e a v) cur_map ->
-    update_cur_version_region lm cur_map (finz.seq_between b e) = Some (lm', cur_map') ->
-    update_version_word_region lm (LCap p b e a v) = Some lm'.
-  Proof.
-    intros Hcur_word Hupd.
-    eapply update_cur_version_region_implies_next_version_gen; eauto.
-    apply finz_seq_between_NoDup.
-  Qed.
-
   Inductive IsUnique_fail (lregs : LReg) (lmem : LMem) (dst src : RegName): Prop :=
   | IsUnique_fail_cap (lwsrc: LWord) :
     lregs !! src = Some lwsrc ->
@@ -90,7 +29,7 @@ Section cap_lang_rules.
   | IsUnique_fail_invalid_PC_true (lwsrc: LWord) p b e a v:
     lregs !! src = Some lwsrc ->
     get_lcap lwsrc = Some (LSCap p b e a v) ->
-    incrementLPC (<[ dst := LInt 1 ]> (<[ src := LCap p b e a (v+1) ]> lregs)) = None ->
+    incrementLPC (<[ dst := LInt 1 ]> (<[ src := next_version_lword lwsrc ]> lregs)) = None ->
     IsUnique_fail lregs lmem dst src
 
   | IsUnique_fail_invalid_PC_false (lwsrc: LWord):
@@ -106,8 +45,8 @@ Section cap_lang_rules.
     lregs !! src = Some lwsrc ->
     get_lcap lwsrc = Some (LSCap p b e a v) ->
     (* we update the region of memory with the new version *)
-    update_version_word_region lmem lwsrc = Some lmem' →
-    incrementLPC (<[ dst := LInt 1 ]> (<[ src := LCap p b e a (v+1) ]> lregs)) = Some lregs' ->
+    update_version_word_region lmem lwsrc = lmem' →
+    incrementLPC (<[ dst := LInt 1 ]> (<[ src := next_version_lword lwsrc ]> lregs)) = Some lregs' ->
     IsUnique_spec lregs lmem dst src lregs' lmem' NextIV
 
   | IsUnique_success_false (lwsrc: LWord) p b e a v :
@@ -124,120 +63,40 @@ Section cap_lang_rules.
     IsUnique_spec lregs lmem dst src lregs' lmem' FailedV
   .
 
+  Definition read_reg_inr' (lregs : LReg) (r : RegName) ot p b e a v :=
+    match lregs !! r with
+      | Some (LCap p' b' e' a' v')
+        => (LCap p' b' e' a' v') = LCap p b e a v
+      | Some (LSealedCap ot' p' b' e' a' v')
+        => (LSealedCap ot' p' b' e' a' v') = (LSealedCap ot p b e a v)
+      | Some _ => True
+      | None => False end.
+
   (* TODO @Bastien rename *)
   Definition allow_access_map_or_true (r : RegName) (lregs : LReg) (lmem : LMem) : Prop :=
-    exists p b e a v, read_reg_inr lregs r p b e a v
-                 ∧ if decide (lregs !! r = Some (LCap p b e a v))
+    exists ot p b e a v, read_reg_inr' lregs r ot p b e a v
+                 ∧ if decide (lregs !! r = Some (LCap p b e a v) \/ lregs !! r = Some (LSealedCap ot p b e a v))
                    then Forall (fun a' => exists lw, lmem !! (a',v) = Some lw) (finz.seq_between b e)
                    else True.
 
   Lemma allow_access_implies_memmap:
-    ∀ (r : RegName) (lmem : LMem) (lregs : LReg) (p : Perm) (b e a : Addr) v,
+    ∀ (r : RegName) (lmem : LMem) (lregs : LReg) (ot : OType) (p : Perm) (b e a : Addr) (v : Version),
       allow_access_map_or_true r lregs lmem
-      → lregs !! r = Some (LCap p b e a v)
+      → (lregs !! r = Some (LCap p b e a v) \/ lregs !! r = Some (LSealedCap ot p b e a v))
+      (* TODO this is too strong, because it forbids the possibility
+         to update a word, even if we own part of the points-to.
+         Do we really need to own all the points-to of the region ?
+         I don't think so.... We just don't get the updated version...
+         I think ? *)
       → Forall ( fun a => exists lw, lmem !! (a,v) = Some lw) (finz.seq_between b e).
   Proof.
-    intros r lmem lregs p b e a v HaAccess Hrv.
-    unfold allow_access_map_or_true, read_reg_inr in HaAccess.
-    destruct HaAccess as (?&?&?&?&?& Hrinr & Hmem).
-    rewrite Hrv in Hrinr. inversion Hrinr; subst.
-    case_decide as Hrega.
-    - exact Hmem.
-    - contradiction Hrega.
-  Qed.
-
-  (* TODO move *)
-  Lemma gen_heap_lmem_version_update :
-    ∀ (lm lmem lm' lmem': LMem) (cur_map cur_map': VMap)
-      (la : list Addr) ( v : Version ),
-    NoDup la ->
-    lmem ⊆ lm ->
-    update_cur_version_region lm cur_map la = Some (lm', cur_map') ->
-    update_cur_version_region lmem cur_map la = Some (lmem', cur_map') ->
-    Forall (λ a : Addr, ∃ lw, lmem !! (a, v) = Some lw) la ->
-    Forall (λ a : Addr, lm !! (a, v+1) = None) la ->
-    Forall (λ a : Addr, cur_map !! a = Some v) la ->
-    gen_heap_interp lm
-    -∗ ([∗ map] k↦y ∈ lmem, mapsto k (DfracOwn 1) y)
-    ==∗ gen_heap_interp lm'
-      ∗ [∗ map] k↦y ∈ lmem', mapsto k (DfracOwn 1) y.
-  Proof.
-    move=> lm lmem lm' lmem' cur_map cur_map' la.
-    move: lm lmem lm' lmem' cur_map cur_map'.
-    induction la as [|a la IH];
-    iIntros
-      (lm lmem lm' lmem' cur_map cur_map' v HNoDup_la Hlmem_incl Hupd_lm Hupd_lmem
-         HmemMap HmemMap_maxv HcurMap)
-        "Hgen Hmem".
-    - (* no addresses updated *)
-      cbn in Hupd_lm, Hupd_lmem ; simplify_eq.
-      iModIntro; iFrame.
-    - cbn in Hupd_lm, Hupd_lmem.
-      apply bind_Some in Hupd_lm, Hupd_lmem.
-
-      destruct Hupd_lm as ((lm0, cur_map0) & Hupd_lm & Hupd_lm_la).
-      rewrite -/(update_cur_version_region lm cur_map la) in Hupd_lm.
-
-      destruct Hupd_lmem as ((lmem1, cur_map1) & Hupd_lmem & Hupd_lmem_la).
-      rewrite -/(update_cur_version_region lmem cur_map la) in Hupd_lmem.
-
-      apply NoDup_cons in HNoDup_la.
-      destruct HNoDup_la as [Ha_not_la HNoDup_la].
-      apply Forall_cons in HmemMap.
-      destruct HmemMap as ([lw Hlmem_la] & HmemMap).
-      apply Forall_cons in HcurMap.
-      destruct HcurMap as (Hcur_la & HcurMap).
-      apply Forall_cons in HmemMap_maxv.
-      destruct HmemMap_maxv as (Hmaxv_lm & HmemMap_maxv).
-
-      pose proof (lookup_weaken _ _ _ _ Hlmem_la Hlmem_incl) as Hlm_la.
-
-      rewrite /update_cur_version_addr in Hupd_lm_la, Hupd_lmem_la.
-      pose proof
-        (update_cur_version_region_notin_preserves_cur_map
-           _ _ _ _ _ _ _ Ha_not_la Hcur_la Hupd_lm)
-        as H0cur_a
-      .
-      pose proof
-        (update_cur_version_region_notin_preserves_cur_map
-           _ _ _ _ _ _ _ Ha_not_la Hcur_la Hupd_lmem)
-        as H1cur_a
-      .
-      rewrite H0cur_a /= in Hupd_lm_la.
-      rewrite H1cur_a /= in Hupd_lmem_la.
-
-      assert (lm0 !! (a,v) = Some lw) as Hlm0_la.
-      { eapply (update_cur_version_region_notin_read_mem lm lm0 cur_map cur_map0)
-      ; eauto.
-      }
-
-      assert (lmem1 !! (a,v) = Some lw) as Hlmem1_la.
-      { eapply (update_cur_version_region_notin_read_mem lmem lmem1 cur_map cur_map1)
-      ; eauto.
-      }
-
-      rewrite /update_version_addr Hlm0_la /= in Hupd_lm_la.
-      rewrite /update_version_addr Hlmem1_la /= in Hupd_lmem_la.
-      simplify_map_eq.
-      rename H3 into Hcur_eq.
-
-      eapply insert_inj in Hcur_eq; simplify_eq ; cycle 1.
-      { by rewrite H0cur_a H1cur_a. }
-
-      assert (lmem !! (a, v + 1) = None) as Hlmem_maxv.
-      { eapply lookup_weaken_None; eauto. }
-      assert (lm0 !! (a, v + 1) = None).
-      { eapply (update_cur_version_region_notin_read_mem lm lm0) ; eauto. }
-      assert (lmem1 !! (a, v + 1) = None).
-      { eapply (update_cur_version_region_notin_read_mem lmem lmem1) ; eauto. }
-
-      iMod (IH lm lmem lm0 lmem1 with "Hgen Hmem") as "[Hgen Hmem]"
-      ; eauto.
-
-      iMod (((gen_heap_alloc lm0 (a, v + 1) lw) with "Hgen"))
-      as "(Hgen & Ha & _)"; auto.
-
-      by iDestruct (big_sepM_insert with "[Ha Hmem]") as "H" ; eauto ; iFrame.
+    intros r lmem lregs ot p b e a v HaAccess Hrv.
+    rewrite /allow_access_map_or_true /read_reg_inr' in HaAccess.
+    destruct HaAccess as (?&?&?&?&?&?& Hrinr & Hmem).
+    destruct Hrv as [Hrv | Hrv].
+    all: rewrite Hrv in Hrinr; inversion Hrinr; subst.
+    all: case_decide as Hrega; [exact Hmem | contradiction Hrega].
+    all: simplify_map_eq; (try by left) ; (try by right).
   Qed.
 
   (** NOTE Proof strategy:
@@ -298,7 +157,7 @@ Section cap_lang_rules.
     (* necessary for update_cur_version... *)
     NoDup (finz.seq_between b e) ->
     update_cur_version_region lm cur_map (finz.seq_between b e)
-    = Some (lm', cur_map') ->
+    = (lm', cur_map') ->
     mem_phys_log_corresponds mem lm cur_map ->
     mem_phys_log_corresponds mem lm' cur_map'.
   Proof.
@@ -361,7 +220,7 @@ Section cap_lang_rules.
     (* Start the different cases now *)
 
     (* src contains a capability *)
-    destruct (is_log_cap lsrcv) eqn:Hlsrcv; cycle 1; subst srcv; cbn in *.
+    destruct (is_lcap lsrcv) eqn:Hlsrcv; cycle 1; subst srcv; cbn in *.
     { (* Fail : not a capability *)
       destruct_lword lsrcv; cbn in * ; try congruence; clear Hlsrcv.
       all: simplify_map_eq.
@@ -372,8 +231,9 @@ Section cap_lang_rules.
     }
     destruct_lword lsrcv; cbn in * ; try congruence; clear Hlsrcv.
 
-    pose proof
-      (allow_access_implies_memmap src lmem lregs p b e a v HaAccess Hlsrc')
+    {
+    opose proof
+      (allow_access_implies_memmap src lmem lregs 0%ot p b e a v HaAccess _)
       as HmemMap ; auto.
 
     (* sweep success or sweep fail *)
@@ -444,211 +304,647 @@ Section cap_lang_rules.
         as HmemMap_maxv.
 
       destruct (update_cur_version_word_region lmem cur_map (LCap p b e a v))
-        as [ [lmem' cur_map']|] eqn:Hupd_lm
-      ; rewrite /update_cur_version_word_region /= in Hupd_lm
+        as [lmem' cur_map'] eqn:Hupd_lmem
+      ; rewrite /update_cur_version_word_region /= in Hupd_lmem
       ; cycle 1.
-      {
-        exfalso.
-        apply eq_None_not_Some in Hupd_lm.
-        apply Hupd_lm.
-        eapply update_cur_version_region_Some; eauto.
-      }
+      (* { *)
+      (*   exfalso. *)
+      (*   apply eq_None_not_Some in Hupd_lmem. *)
+      (*   apply Hupd_lm. *)
+      (*   eapply update_cur_version_region_Some; eauto. *)
+      (* } *)
 
-      pose proof Hupd_lm as Hupd_lmem.
-      eapply update_cur_version_region_mono in Hupd_lmem ; eauto.
-      destruct Hupd_lmem as (lm' & Hupd_lmem & Hmem').
+      pose proof Hupd_lmem as Hupd_lm.
+      eapply update_cur_version_region_mono in Hupd_lm ; eauto.
+      destruct Hupd_lm as (lm' & Hupd_lm & Hmem').
+
+      Set Nested Proofs Allowed.
+      Lemma gen_heap_lmem_version_update `{HmemG : memG Σ, HregG : regG Σ} :
+        ∀ (lm lmem lm' lmem': LMem) (cur_map cur_map': VMap)
+          (la : list Addr) ( v : Version ),
+          NoDup la ->
+          lmem ⊆ lm ->
+          update_cur_version_region lm cur_map la = (lm', cur_map') ->
+          update_cur_version_region lmem cur_map la = (lmem', cur_map') ->
+          Forall (λ a : Addr, ∃ lw, lmem !! (a, v) = Some lw) la ->
+          Forall (λ a : Addr, lm !! (a, v+1) = None) la ->
+          Forall (λ a : Addr, cur_map !! a = Some v) la ->
+          (* Forall (λ a : Addr, (forall va, cur_map !! a = Some va <-> is_Some (lmem !! (a,va)))) la -> *)
+          (* Forall (λ a : Addr, (forall va, cur_map !! a = Some va <-> is_Some (lm !! (a,va)))) la -> *)
+          gen_heap_interp lm
+          -∗ ([∗ map] k↦y ∈ lmem, mapsto k (DfracOwn 1) y)
+          ==∗ gen_heap_interp lm'
+              ∗ [∗ map] k↦y ∈ lmem', mapsto k (DfracOwn 1) y.
+    Proof.
+    Admitted.
+
 
       iMod ((gen_heap_lmem_version_update lm lmem lm' lmem' ) with "Hm Hmem")
-        as "[Hm Hmem]"; eauto.
+        as "[Hm Hmem]". eauto.
 
-      assert (update_version_word_region lmem (LCap p b e a v) = Some lmem').
-      {
-        eapply update_cur_version_region_implies_next_version; eauto.
-        destruct HLinv as [Hinv_reg _].
-        eapply lreg_read_iscur; eauto.
-      }
+    (*   assert (update_version_word_region lmem (LCap p b e a v) = Some lmem'). *)
+    (*   { *)
+    (*     eapply update_cur_version_region_implies_next_version; eauto. *)
+    (*     destruct HLinv as [Hinv_reg _]. *)
+    (*     eapply lreg_read_iscur; eauto. *)
+    (*   } *)
 
-      (* we destruct the cases when the registers are equals *)
-      destruct (decide (src = PC)); simplify_map_eq ; cycle 1.
-      * (* src <> PC *)
-        destruct (decide (src = dst)) ; simplify_map_eq ; cycle 1.
-        ** (* src <> dst *)
-          iMod ((gen_heap_update_inSepM _ _ src (LCap p b e a (v + 1))) with "Hr Hmap")
-            as "[Hr Hmap]"; eauto.
-          iMod ((gen_heap_update_inSepM _ _ dst (LInt 1)) with "Hr Hmap")
-            as "[Hr Hmap]"; eauto ; first by simplify_map_eq.
-          iMod ((gen_heap_update_inSepM _ _ PC (LCap p1 b1 e1 a_pc1 v1)) with "Hr Hmap")
-            as "[Hr Hmap]"; eauto ; first by simplify_map_eq.
+    (*   (* we destruct the cases when the registers are equals *) *)
+    (*   destruct (decide (src = PC)); simplify_map_eq ; cycle 1. *)
+    (*   * (* src <> PC *) *)
+    (*     destruct (decide (src = dst)) ; simplify_map_eq ; cycle 1. *)
+    (*     ** (* src <> dst *) *)
+    (*       iMod ((gen_heap_update_inSepM _ _ src (LCap p b e a (v + 1))) with "Hr Hmap") *)
+    (*         as "[Hr Hmap]"; eauto. *)
+    (*       iMod ((gen_heap_update_inSepM _ _ dst (LInt 1)) with "Hr Hmap") *)
+    (*         as "[Hr Hmap]"; eauto ; first by simplify_map_eq. *)
+    (*       iMod ((gen_heap_update_inSepM _ _ PC (LCap p1 b1 e1 a_pc1 v1)) with "Hr Hmap") *)
+    (*         as "[Hr Hmap]"; eauto ; first by simplify_map_eq. *)
 
-          iFrame; iModIntro ; iSplitR "Hφ Hmap Hmem"
-          ; [| iApply "Hφ" ; iFrame; iPureIntro; econstructor; eauto].
-          iExists _, lm', cur_map'; iFrame; auto
-          ; iPureIntro; econstructor; eauto
-          ; destruct HLinv as [Hreg_inv Hmem_inv]
-          ; cbn in *.
-          {
-            rewrite (insert_commute _ _ src) // (insert_commute _ _ src) //.
-            eapply lookup_weaken in HPC'' ; eauto.
-            replace reg with (<[ src := WCap p b e a ]> reg).
-            2: { rewrite insert_id;auto. }
-            do 2 (rewrite (insert_commute _ _ src) //).
+    (*       iFrame; iModIntro ; iSplitR "Hφ Hmap Hmem" *)
+    (*       ; [| iApply "Hφ" ; iFrame; iPureIntro; econstructor; eauto]. *)
+    (*       iExists _, lm', cur_map'; iFrame; auto *)
+    (*       ; iPureIntro; econstructor; eauto *)
+    (*       ; destruct HLinv as [Hreg_inv Hmem_inv] *)
+    (*       ; cbn in *. *)
+    (*       { *)
+    (*         rewrite (insert_commute _ _ src) // (insert_commute _ _ src) //. *)
+    (*         eapply lookup_weaken in HPC'' ; eauto. *)
+    (*         replace reg with (<[ src := WCap p b e a ]> reg). *)
+    (*         2: { rewrite insert_id;auto. } *)
+    (*         do 2 (rewrite (insert_commute _ _ src) //). *)
 
-            eapply update_cur_version_reg_phys_log_cor_updates_src with
-            (phm := mem).
-            eapply update_cur_version_region_update_lcap; eauto.
-            eapply lreg_read_iscur; eauto.
-            2: by rewrite lookup_insert_ne // lookup_insert_ne //.
-            2: {
-              eapply unique_in_machineL_insert_reg; eauto ; try by simplify_map_eq.
-              eapply not_overlap_word_leaL with (a2' := a1); eauto.
-              eapply (unique_in_machineL_not_overlap_word _ _ src PC); eauto.
+    (*         eapply update_cur_version_reg_phys_log_cor_updates_src with *)
+    (*         (phm := mem). *)
+    (*         eapply update_cur_version_region_update_lcap; eauto. *)
+    (*         eapply lreg_read_iscur; eauto. *)
+    (*         2: by rewrite lookup_insert_ne // lookup_insert_ne //. *)
+    (*         2: { *)
+    (*           eapply unique_in_machineL_insert_reg; eauto ; try by simplify_map_eq. *)
+    (*           eapply not_overlap_word_leaL with (a2' := a1); eauto. *)
+    (*           eapply (unique_in_machineL_not_overlap_word _ _ src PC); eauto. *)
 
-              eapply unique_in_machineL_insert_reg; eauto
-              ; try by simplify_map_eq.
-            }
-            split; eauto.
-            eapply lreg_insert_respects_corresponds; eauto.
-            eapply lreg_insert_respects_corresponds; eauto.
-            by cbn.
-            apply is_cur_word_lea with (a := a1).
-            eapply lreg_read_iscur; eauto.
-            eauto.
-          }
-          { eapply mem_phys_log_update ; eauto. }
+    (*           eapply unique_in_machineL_insert_reg; eauto *)
+    (*           ; try by simplify_map_eq. *)
+    (*         } *)
+    (*         split; eauto. *)
+    (*         eapply lreg_insert_respects_corresponds; eauto. *)
+    (*         eapply lreg_insert_respects_corresponds; eauto. *)
+    (*         by cbn. *)
+    (*         apply is_cur_word_lea with (a := a1). *)
+    (*         eapply lreg_read_iscur; eauto. *)
+    (*         eauto. *)
+    (*       } *)
+    (*       { eapply mem_phys_log_update ; eauto. } *)
 
-        ** (* src = dst *)
-          iMod ((gen_heap_update_inSepM _ _ dst (LInt 1)) with "Hr Hmap")
-            as "[Hr Hmap]"; eauto.
-          iMod ((gen_heap_update_inSepM _ _ PC (LCap p1 b1 e1 a_pc1 v1)) with "Hr Hmap")
-            as "[Hr Hmap]"; eauto ; first by simplify_map_eq.
+    (*     ** (* src = dst *) *)
+    (*       iMod ((gen_heap_update_inSepM _ _ dst (LInt 1)) with "Hr Hmap") *)
+    (*         as "[Hr Hmap]"; eauto. *)
+    (*       iMod ((gen_heap_update_inSepM _ _ PC (LCap p1 b1 e1 a_pc1 v1)) with "Hr Hmap") *)
+    (*         as "[Hr Hmap]"; eauto ; first by simplify_map_eq. *)
 
-          iFrame; iModIntro ; iSplitR "Hφ Hmap Hmem"
-          ; [| iApply "Hφ" ; iFrame; iPureIntro; econstructor; eauto].
-          2: { rewrite insert_insert in H'lregs'.
-               rewrite insert_insert. done.
-          }
-          iExists _, lm', cur_map'; iFrame; auto
-          ; iPureIntro; econstructor; eauto
-          ; destruct HLinv as [Hreg_inv Hmem_inv]
-          ; cbn in *.
-          {
-            rewrite (insert_commute _ _ dst) // (insert_commute _ _ dst) //.
-            assert (HPC' := lookup_weaken _ _ _ _ HPC'' Hregs).
+    (*       iFrame; iModIntro ; iSplitR "Hφ Hmap Hmem" *)
+    (*       ; [| iApply "Hφ" ; iFrame; iPureIntro; econstructor; eauto]. *)
+    (*       2: { rewrite insert_insert in H'lregs'. *)
+    (*            rewrite insert_insert. done. *)
+    (*       } *)
+    (*       iExists _, lm', cur_map'; iFrame; auto *)
+    (*       ; iPureIntro; econstructor; eauto *)
+    (*       ; destruct HLinv as [Hreg_inv Hmem_inv] *)
+    (*       ; cbn in *. *)
+    (*       { *)
+    (*         rewrite (insert_commute _ _ dst) // (insert_commute _ _ dst) //. *)
+    (*         assert (HPC' := lookup_weaken _ _ _ _ HPC'' Hregs). *)
 
-            eapply update_cur_version_reg_phys_log_cor_updates_src
-              with (phm := mem) ; eauto.
-            done.
-            2: by rewrite lookup_insert_ne // lookup_insert_ne //.
-            2: {
-              eapply unique_in_machineL_insert_reg; eauto ; try by simplify_map_eq.
-              eapply not_overlap_word_leaL with (a2' := a1); eauto.
-              eapply (unique_in_machineL_not_overlap_word _ lr dst); eauto.
-            }
-            split; eauto.
-            eapply lreg_insert_respects_corresponds; eauto.
-            apply is_cur_word_lea with (a := a1).
-            eapply lreg_read_iscur; eauto.
-          }
-          { eapply mem_phys_log_update ; eauto. }
+    (*         eapply update_cur_version_reg_phys_log_cor_updates_src *)
+    (*           with (phm := mem) ; eauto. *)
+    (*         done. *)
+    (*         2: by rewrite lookup_insert_ne // lookup_insert_ne //. *)
+    (*         2: { *)
+    (*           eapply unique_in_machineL_insert_reg; eauto ; try by simplify_map_eq. *)
+    (*           eapply not_overlap_word_leaL with (a2' := a1); eauto. *)
+    (*           eapply (unique_in_machineL_not_overlap_word _ lr dst); eauto. *)
+    (*         } *)
+    (*         split; eauto. *)
+    (*         eapply lreg_insert_respects_corresponds; eauto. *)
+    (*         apply is_cur_word_lea with (a := a1). *)
+    (*         eapply lreg_read_iscur; eauto. *)
+    (*       } *)
+    (*       { eapply mem_phys_log_update ; eauto. } *)
 
-      * (* src = PC *)
-        rewrite (insert_commute _ dst PC) //= insert_insert insert_commute //= in H'lregs'.
-        (* we update the registers with their new value *)
-        destruct (decide (dst = PC)) ; simplify_map_eq.
-        (* dst ≠ PC *)
-        iMod ((gen_heap_update_inSepM _ _ dst ) with "Hr Hmap") as "[Hr Hmap]"; eauto.
-        iMod ((gen_heap_update_inSepM _ _ PC ) with "Hr Hmap") as "[Hr Hmap]"; eauto
-        ; first by simplify_map_eq.
+    (*   * (* src = PC *) *)
+    (*     rewrite (insert_commute _ dst PC) //= insert_insert insert_commute //= in H'lregs'. *)
+    (*     (* we update the registers with their new value *) *)
+    (*     destruct (decide (dst = PC)) ; simplify_map_eq. *)
+    (*     (* dst ≠ PC *) *)
+    (*     iMod ((gen_heap_update_inSepM _ _ dst ) with "Hr Hmap") as "[Hr Hmap]"; eauto. *)
+    (*     iMod ((gen_heap_update_inSepM _ _ PC ) with "Hr Hmap") as "[Hr Hmap]"; eauto *)
+    (*     ; first by simplify_map_eq. *)
 
-        iFrame; iModIntro ; iSplitR "Hφ Hmap Hmem"
-        ; [| iApply "Hφ" ; iFrame; iPureIntro; econstructor; eauto].
-        iExists _, lm', cur_map'; iFrame; auto
-        ; iPureIntro; econstructor; eauto
-        ; destruct HLinv as [Hreg_inv Hmem_inv]
-        ; cbn in *.
-        {
+    (*     iFrame; iModIntro ; iSplitR "Hφ Hmap Hmem" *)
+    (*     ; [| iApply "Hφ" ; iFrame; iPureIntro; econstructor; eauto]. *)
+    (*     iExists _, lm', cur_map'; iFrame; auto *)
+    (*     ; iPureIntro; econstructor; eauto *)
+    (*     ; destruct HLinv as [Hreg_inv Hmem_inv] *)
+    (*     ; cbn in *. *)
+    (*     { *)
+    (*         eapply update_cur_version_reg_phys_log_cor_updates_src with *)
+    (*         (phm := mem). *)
+    (*         eapply update_cur_version_region_update_lcap ; eauto. *)
+    (*         apply is_cur_word_lea with (a := a1). *)
+    (*         eapply lreg_read_iscur; eauto. *)
+    (*         2: by rewrite lookup_insert_ne // lookup_insert_ne //. *)
+    (*         2: { *)
+    (*           eapply unique_in_machineL_insert_reg; eauto ; try by simplify_map_eq. *)
+    (*         } *)
+    (*         split; eauto. *)
+    (*         eapply lreg_insert_respects_corresponds; eauto. *)
+    (*         by cbn. *)
+    (*         eapply Hupd_lmem. *)
+    (*       } *)
+    (*     { eapply mem_phys_log_update ; eauto. } *)
 
-            eapply update_cur_version_reg_phys_log_cor_updates_src with
-            (phm := mem).
-            eapply update_cur_version_region_update_lcap ; eauto.
-            apply is_cur_word_lea with (a := a1).
-            eapply lreg_read_iscur; eauto.
-            2: by rewrite lookup_insert_ne // lookup_insert_ne //.
-            2: {
-              eapply unique_in_machineL_insert_reg; eauto ; try by simplify_map_eq.
-            }
-            split; eauto.
-            eapply lreg_insert_respects_corresponds; eauto.
-            by cbn.
-            eapply Hupd_lmem.
-          }
-        { eapply mem_phys_log_update ; eauto. }
+    (* - (* sweep = false *) *)
 
-    - (* sweep = false *)
+    (*   destruct (incrementLPC (<[ dst := LInt 0 ]> lregs)) *)
+    (*     as  [ lregs' |] eqn:Hlregs' *)
+    (*   ; pose proof Hlregs' as H'lregs' *)
+    (*   ; cycle 1. *)
+    (*   {  (* Failure: the PC could not be incremented correctly *) *)
+    (*     apply incrementLPC_fail_updatePC with (m:=mem) (etbl:=etable) (ecur:=enumcur) in Hlregs'. *)
+    (*     eapply updatePC_fail_incl with (m':=mem) (etbl':=etable) (ecur':=enumcur) in Hlregs'. *)
+    (*     2: { *)
+    (*       rewrite /lreg_strip lookup_fmap. *)
+    (*       apply fmap_is_Some. *)
+    (*       destruct (decide (dst = PC)) ; simplify_map_eq; auto. *)
+    (*     } *)
+    (*     2: apply map_fmap_mono ; apply insert_mono ; eauto. *)
+    (*     replace ((λ lw : LWord, lword_get_word lw) <$> (<[dst:=LInt 0]> lr)) *)
+    (*       with (<[dst:= WInt 0]> reg) *)
+    (*       in Hlregs' *)
+    (*     ; cycle 1. *)
+    (*     { destruct HLinv as [ [Hstrips Hcurreg] _]. *)
+    (*       rewrite -Hstrips !fmap_insert -/(lreg_strip lr) //=. *)
+    (*     } *)
 
-      destruct (incrementLPC (<[ dst := LInt 0 ]> lregs))
-        as  [ lregs' |] eqn:Hlregs'
-      ; pose proof Hlregs' as H'lregs'
-      ; cycle 1.
-      {  (* Failure: the PC could not be incremented correctly *)
-        apply incrementLPC_fail_updatePC with (m:=mem) (etbl:=etable) (ecur:=enumcur) in Hlregs'.
-        eapply updatePC_fail_incl with (m':=mem) (etbl':=etable) (ecur':=enumcur) in Hlregs'.
-        2: {
-          rewrite /lreg_strip lookup_fmap.
-          apply fmap_is_Some.
-          destruct (decide (dst = PC)) ; simplify_map_eq; auto.
-        }
-        2: apply map_fmap_mono ; apply insert_mono ; eauto.
-        replace ((λ lw : LWord, lword_get_word lw) <$> (<[dst:=LInt 0]> lr))
-          with (<[dst:= WInt 0]> reg)
-          in Hlregs'
-        ; cycle 1.
-        { destruct HLinv as [ [Hstrips Hcurreg] _].
-          rewrite -Hstrips !fmap_insert -/(lreg_strip lr) //=.
-        }
+    (*     rewrite Hlregs' in Hstep. inversion Hstep. *)
+    (*     iSplitR "Hφ Hmap Hmem" *)
+    (*     ; [ iExists lr, lm, cur_map; iFrame; auto *)
+    (*       | iApply "Hφ" ; iFrame ; iFailCore IsUnique_fail_invalid_PC_false *)
+    (*       ]. *)
+    (*   } *)
 
-        rewrite Hlregs' in Hstep. inversion Hstep.
-        iSplitR "Hφ Hmap Hmem"
-        ; [ iExists lr, lm, cur_map; iFrame; auto
-          | iApply "Hφ" ; iFrame ; iFailCore IsUnique_fail_invalid_PC_false
-          ].
-      }
+    (*   (* PC has been incremented correctly *) *)
+    (*   rewrite /update_reg /= in Hstep. *)
+    (*   eapply (incrementLPC_success_updatePC _ mem etable enumcur) in Hlregs' *)
+    (*       as (p1 & b1 & e1 & a1 & a_pc1 & v1 & HPC'' & Ha_pc' & HuPC & ->) *)
+    (*   ; simplify_map_eq. *)
+    (*   assert (dst <> PC) as Hdst by (intro ; simplify_map_eq). *)
+    (*   eapply updatePC_success_incl with (m':=mem) (etbl':=etable) (ecur':=enumcur) in HuPC. *)
+    (*   2: apply map_fmap_mono ; apply insert_mono ; eauto. *)
+    (*   replace ((λ lw, lword_get_word lw) <$> <[dst:=LInt 0]> lr) *)
+    (*     with (<[dst:=WInt 0]> reg) in HuPC. *)
+    (*   2: { destruct HLinv as [ [Hstrips Hcurreg] _] *)
+    (*        ; rewrite -Hstrips !fmap_insert -/(lreg_strip lr) //=. *)
+    (*   } *)
+    (*   rewrite HuPC in Hstep; clear HuPC. *)
+    (*   inversion Hstep; clear Hstep ; simplify_map_eq. *)
 
-      (* PC has been incremented correctly *)
-      rewrite /update_reg /= in Hstep.
-      eapply (incrementLPC_success_updatePC _ mem etable enumcur) in Hlregs'
-          as (p1 & b1 & e1 & a1 & a_pc1 & v1 & HPC'' & Ha_pc' & HuPC & ->)
-      ; simplify_map_eq.
-      assert (dst <> PC) as Hdst by (intro ; simplify_map_eq).
-      eapply updatePC_success_incl with (m':=mem) (etbl':=etable) (ecur':=enumcur) in HuPC.
-      2: apply map_fmap_mono ; apply insert_mono ; eauto.
-      replace ((λ lw, lword_get_word lw) <$> <[dst:=LInt 0]> lr)
-        with (<[dst:=WInt 0]> reg) in HuPC.
-      2: { destruct HLinv as [ [Hstrips Hcurreg] _]
-           ; rewrite -Hstrips !fmap_insert -/(lreg_strip lr) //=.
-      }
-      rewrite HuPC in Hstep; clear HuPC.
-      inversion Hstep; clear Hstep ; simplify_map_eq.
+    (*   iMod ((gen_heap_update_inSepM _ _ dst ) with "Hr Hmap") as "[Hr Hmap]"; eauto. *)
+    (*   iMod ((gen_heap_update_inSepM _ _ PC ) with "Hr Hmap") as "[Hr Hmap]"; eauto *)
+    (*   ; first by simplify_map_eq. *)
 
-      iMod ((gen_heap_update_inSepM _ _ dst ) with "Hr Hmap") as "[Hr Hmap]"; eauto.
-      iMod ((gen_heap_update_inSepM _ _ PC ) with "Hr Hmap") as "[Hr Hmap]"; eauto
-      ; first by simplify_map_eq.
+    (*   iFrame; iModIntro ; iSplitR "Hφ Hmap Hmem" *)
+    (*   ; [| iApply "Hφ" ; iFrame; iPureIntro; eapply IsUnique_success_false ; eauto]. *)
 
-      iFrame; iModIntro ; iSplitR "Hφ Hmap Hmem"
-      ; [| iApply "Hφ" ; iFrame; iPureIntro; eapply IsUnique_success_false ; eauto].
+    (*   iExists _, lm, cur_map; iFrame; auto *)
+    (*   ; iPureIntro; econstructor; eauto *)
+    (*   ; destruct HLinv as [ [Hstrips Hcur_reg] [Hdom Hroot] ] *)
+    (*   ; cbn in * *)
+    (*   ; [|split;eauto] *)
+    (*   . *)
+    (*   split; first by rewrite -Hstrips /lreg_strip !fmap_insert /=. *)
+    (*   apply map_Forall_insert_2 ; [|by apply map_Forall_insert_2; cbn]. *)
+    (*   rewrite HPC in HPC'' ; simplify_eq. *)
+    (*   eapply is_cur_word_cap_change; eauto. *)
+    (*   Unshelve. all: eauto. *)
+    (*   } *)
 
-      iExists _, lm, cur_map; iFrame; auto
-      ; iPureIntro; econstructor; eauto
-      ; destruct HLinv as [ [Hstrips Hcur_reg] [Hdom Hroot] ]
-      ; cbn in *
-      ; [|split;eauto]
-      .
-      split; first by rewrite -Hstrips /lreg_strip !fmap_insert /=.
-      apply map_Forall_insert_2 ; [|by apply map_Forall_insert_2; cbn].
-      rewrite HPC in HPC'' ; simplify_eq.
-      eapply is_cur_word_cap_change; eauto.
-      Unshelve. all: eauto.
-  Qed.
+    (*   { *)
+    (*     opose proof *)
+    (*       (allow_access_implies_memmap src lmem lregs o p b e a v HaAccess _) *)
+    (*       as HmemMap ; auto. *)
+
+    (*     (* sweep success or sweep fail *) *)
+    (*     destruct (sweep mem reg src) as [|] eqn:Hsweep ; cbn in Hstep. *)
+    (*     - (* sweep is true *) *)
+    (*       eapply sweep_true_specL in Hsweep; eauto. *)
+
+    (*       destruct (incrementLPC (<[ dst := LInt 1 ]> *)
+    (*                                 (<[ src := LSealedCap o p b e a (v + 1)]> lregs))) *)
+    (*         as  [ lregs' |] eqn:Hlregs' *)
+    (*       ; pose proof Hlregs' as H'lregs' *)
+    (*       ; cycle 1. *)
+    (*       { (* Failure: the PC could not be incremented correctly *) *)
+    (*         apply incrementLPC_fail_updatePC with (m:=mem) (etbl:=etable) (ecur:=enumcur) in Hlregs'. *)
+    (*         eapply updatePC_fail_incl with (m':=mem) (etbl':=etable) (ecur':=enumcur) in Hlregs'. *)
+    (*         2: { *)
+    (*           rewrite /lreg_strip lookup_fmap. *)
+    (*           apply fmap_is_Some. *)
+    (*           destruct (decide (dst = PC)) ;  destruct (decide (src = PC)) ; simplify_map_eq; auto. *)
+    (*         } *)
+    (*         2: apply map_fmap_mono *)
+    (*         ; apply (insert_mono _ ( <[src:=LSealedCap o p b e a (v + 1)]> lr)) *)
+    (*         ; apply insert_mono ; eauto. *)
+    (*         simplify_pair_eq. *)
+    (*         replace ((λ lw : LWord, lword_get_word lw) <$> (<[dst:=LInt 1]> (<[src:=LSealedCap o p b e a (v + 1)]> lr))) *)
+    (*           with (<[dst:= WInt 1]> reg) *)
+    (*           in Hlregs' *)
+    (*         ; cycle 1. *)
+    (*         { destruct HLinv as [ [Hstrips Hcurreg] _]. *)
+    (*           rewrite -Hstrips !fmap_insert -/(lreg_strip lr) //=. *)
+    (*           rewrite -/(lword_get_word (LSealedCap o p b e a v)). *)
+    (*           erewrite insert_reg_lreg_strip; eauto. *)
+    (*         } *)
+    (*         rewrite Hlregs' in Hstep. inversion Hstep. *)
+    (*         iSplitR "Hφ Hmap Hmem" *)
+    (*         ; [ iExists lr, lm, cur_map; iFrame; auto *)
+    (*           | iApply "Hφ" ; iFrame ; iFailCore IsUnique_fail_invalid_PC_true *)
+    (*           ]. *)
+    (*       } *)
+
+    (*       (* PC has been incremented correctly *) *)
+    (*       rewrite /update_reg /= in Hstep. *)
+    (*       eapply (incrementLPC_success_updatePC _ mem etable enumcur) in Hlregs' *)
+    (*           as (p1 & b1 & e1 & a1 & a_pc1 & v1 & HPC'' & Ha_pc' & HuPC & ->) *)
+    (*       ; simplify_map_eq. *)
+    (*       assert (dst <> PC) as Hdst by (intro ; simplify_map_eq). *)
+    (*       assert (src <> PC) as Hsrc_neq_pc by (intro ; simplify_map_eq). *)
+    (*       eapply updatePC_success_incl with (m':=mem) (etbl':=etable) (ecur':=enumcur) in HuPC. *)
+    (*       2: apply map_fmap_mono *)
+    (*       ; apply (insert_mono _ ( <[src:=LSealedCap o p b e a (v + 1)]> lr)) *)
+    (*       ; apply insert_mono ; eauto. *)
+    (*       replace ((λ lw, lword_get_word lw) <$> *)
+    (*                <[dst:=LInt 1]> (<[src:=LSealedCap o p b e a (v + 1)]> lr)) *)
+    (*         with (<[dst:=WInt 1]> reg) in HuPC. *)
+    (*       2: { destruct HLinv as [ [Hstrips Hcurreg] _] *)
+    (*            ; rewrite -Hstrips !fmap_insert -/(lreg_strip lr) //=. *)
+    (*            rewrite -/(lword_get_word (LSealedCap o p b e a v)). *)
+    (*            erewrite insert_reg_lreg_strip; eauto. *)
+    (*       } *)
+    (*       rewrite HuPC in Hstep; clear HuPC. *)
+    (*       inversion Hstep; clear Hstep ; simplify_map_eq. *)
+
+    (*       (* update version number of memory points-to *) *)
+    (*       assert (HNoDup : NoDup (finz.seq_between b e)) by (apply finz_seq_between_NoDup). *)
+
+    (*       Set Nested Proofs Allowed. *)
+    (*       Lemma state_phys_log_scap_all_current *)
+    (*         (phr : Reg) (phm : Mem) (lm : LMem) (lr : LReg) (cur_map : VMap) *)
+    (*         (src : RegName) (o : OType) (p : Perm) (b e a : Addr) (v : Version) : *)
+    (*         state_phys_log_corresponds phr phm lr lm cur_map -> *)
+    (*         lr !! src = Some (LSealedCap o p b e a v) -> *)
+    (*         Forall (λ a0 : Addr, cur_map !! a0 = Some v) (finz.seq_between b e). *)
+    (*       Proof. *)
+    (*         move=> [ [_ Hreg_current] Hmem_inv] Hlr_src. *)
+    (*         pose proof (map_Forall_lookup_1 _ _ _ _ Hreg_current Hlr_src) as Hcur_src. *)
+    (*         cbn in *. *)
+    (*         by eapply Forall_forall. *)
+    (*       Qed. *)
+
+    (*       Lemma state_phys_log_last_version_s *)
+    (*         (phr : Reg) (phm : Mem) (lm : LMem) (lr : LReg) (cur_map : VMap) *)
+    (*         (src : RegName) (o : OType) (p : Perm) (b e a : Addr) (v : Version) : *)
+    (*         state_phys_log_corresponds phr phm lr lm cur_map -> *)
+    (*         lr !! src = Some (LSealedCap o p b e a v) -> *)
+    (*         Forall (λ a0 : Addr, lm !! (a0, v+1) = None) (finz.seq_between b e). *)
+    (*       Proof. *)
+    (*         move=> [ [_ Hreg_current] Hmem_inv] Hlr_src. *)
+    (*         pose proof (map_Forall_lookup_1 _ _ _ _ Hreg_current Hlr_src) as Hcur_src. *)
+    (*         cbn in *. *)
+    (*         apply Forall_forall. *)
+    (*         intros a0 Ha0_inbounds. *)
+    (*         apply Hcur_src in Ha0_inbounds. *)
+    (*         assert (is_cur_addr (a0, v) cur_map) as Hcur_a0 by done. *)
+
+    (*         destruct (lm !! (a0, v + 1)) eqn:Hv'. 2: done. *)
+    (*         destruct Hmem_inv as [Hroot Hcur]. *)
+    (*         eapply map_Forall_lookup_1 in Hroot; eauto. *)
+    (*         destruct Hroot as (cur_v & Hcur_v & cur & Hsome & Hmaxv). *)
+    (*         cbn in *. *)
+
+    (*         eapply map_Forall_lookup_1 in Hcur; eauto. *)
+    (*         destruct Hcur as (lw & Hlm & _) ; cbn in *. *)
+    (*         eapply is_cur_addr_same in Hcur_a0; eauto; simplify_eq. *)
+    (*         lia. *)
+    (*       Qed. *)
+
+    (*       pose proof *)
+    (*         (state_phys_log_scap_all_current _ _ _ _ _ _ _ _ _ _ _ _ HLinv Hlsrc) *)
+    (*         as HcurMap. *)
+    (*       pose proof *)
+    (*         (state_phys_log_last_version_s _ _ _ _ _ _ _ _ _ _ _ _ HLinv Hlsrc) *)
+    (*         as HmemMap_maxv. *)
+
+    (*       destruct (update_cur_version_word_region lmem cur_map (LCap p b e a v)) *)
+    (*         as [ [lmem' cur_map']|] eqn:Hupd_lm *)
+    (*       ; rewrite /update_cur_version_word_region /= in Hupd_lm *)
+    (*       ; cycle 1. *)
+    (*       { *)
+    (*         exfalso. *)
+    (*         apply eq_None_not_Some in Hupd_lm. *)
+    (*         apply Hupd_lm. *)
+    (*         eapply update_cur_version_region_Some; eauto. *)
+    (*       } *)
+
+    (*       pose proof Hupd_lm as Hupd_lmem. *)
+    (*       eapply update_cur_version_region_mono in Hupd_lmem ; eauto. *)
+    (*       destruct Hupd_lmem as (lm' & Hupd_lmem & Hmem'). *)
+
+    (*       iMod ((gen_heap_lmem_version_update lm lmem lm' lmem' ) with "Hm Hmem") *)
+    (*         as "[Hm Hmem]"; eauto. *)
+
+    (*       assert (update_version_word_region lmem (LSealedCap o p b e a v) = Some lmem'). *)
+    (*       { *)
+    (*         Lemma update_cur_version_region_implies_next_version_s *)
+    (*           (lm lm' : LMem) (cur_map cur_map': VMap) *)
+    (*           (o : OType) (p : Perm) (b e a : Addr) (v : Version) : *)
+    (*           is_cur_word (LSealedCap o p b e a v) cur_map -> *)
+    (*           update_cur_version_region lm cur_map (finz.seq_between b e) = Some (lm', cur_map') -> *)
+    (*           update_version_word_region lm (LSealedCap o p b e a v) = Some lm'. *)
+    (*         Proof. *)
+    (*           intros Hcur_word Hupd. *)
+    (*           eapply update_cur_version_region_implies_next_version_gen; eauto. *)
+    (*           apply finz_seq_between_NoDup. *)
+    (*         Qed. *)
+    (*         eapply update_cur_version_region_implies_next_version_s; eauto. *)
+    (*         destruct HLinv as [Hinv_reg _]. *)
+    (*         eapply lreg_read_iscur; eauto. *)
+    (*       } *)
+
+    (*       destruct (decide (src = dst)) ; simplify_map_eq ; cycle 1. *)
+    (*       * (* src <> dst *) *)
+    (*           iMod ((gen_heap_update_inSepM _ _ src (LSealedCap o p b e a (v + 1))) with "Hr Hmap") *)
+    (*             as "[Hr Hmap]"; eauto. *)
+    (*           iMod ((gen_heap_update_inSepM _ _ dst (LInt 1)) with "Hr Hmap") *)
+    (*             as "[Hr Hmap]"; eauto ; first by simplify_map_eq. *)
+    (*           iMod ((gen_heap_update_inSepM _ _ PC (LCap p1 b1 e1 a_pc1 v1)) with "Hr Hmap") *)
+    (*             as "[Hr Hmap]"; eauto ; first by simplify_map_eq. *)
+
+    (*           iFrame; iModIntro ; iSplitR "Hφ Hmap Hmem" *)
+    (*           ; [| iApply "Hφ" ; iFrame; iPureIntro; econstructor; eauto]. *)
+    (*           iExists _, lm', cur_map'; iFrame; auto *)
+    (*           ; iPureIntro; econstructor; eauto *)
+    (*           ; destruct HLinv as [Hreg_inv Hmem_inv] *)
+    (*           ; cbn in *. *)
+    (*           { *)
+    (*             rewrite (insert_commute _ _ src) // (insert_commute _ _ src) //. *)
+    (*             eapply lookup_weaken in HPC'' ; eauto. *)
+    (*             replace reg with (<[ src := WSealed o (SCap p b e a) ]> reg). *)
+    (*             2: { rewrite insert_id;auto. } *)
+    (*             do 2 (rewrite (insert_commute _ _ src) //). *)
+
+    (*             Lemma update_cur_version_reg_phys_log_cor_updates_src_s *)
+    (*               (phr : Reg) (phm : Mem) (lr : LReg) (lm lm' : LMem) (cur_map cur_map' : VMap) *)
+    (*               (src : RegName) (o : OType) (p : Perm) (b e a : Addr) ( v : Version ) (lw : LWord) : *)
+    (*               is_cur_word lw cur_map' -> *)
+    (*               state_phys_log_corresponds phr phm lr lm cur_map -> *)
+    (*               lr !! src = Some (LSealedCap o p b e a v) -> *)
+    (*               unique_in_machineL lm lr src (LSealedCap o p b e a v) -> *)
+    (*               update_cur_version_region lm cur_map (finz.seq_between b e) *)
+    (*               = Some (lm', cur_map') -> *)
+    (*               reg_phys_log_corresponds (<[src:= (lword_get_word lw)]> phr) (<[src:= lw]> lr) cur_map'. *)
+    (*             Proof. *)
+    (*               move=> Hcur_lw [Hreg_inv Hmem_inv] Hlr_src Hunique Hupd. *)
+    (*               split. *)
+    (*               - rewrite /lreg_strip fmap_insert /= -/(lreg_strip lr). *)
+    (*                 by replace phr with (lreg_strip lr) by (by destruct Hreg_inv as [? _]). *)
+    (*               - rewrite -insert_delete_insert. *)
+    (*                 eapply lreg_insert_respects_corresponds with (phr := (delete src phr)). *)
+    (*                 2: { by cbn. } *)
+    (*                 destruct Hreg_inv as [Hstrip Hcur_reg]. *)
+    (*                 split. *)
+    (*                 + by rewrite /lreg_strip fmap_delete -/(lreg_strip lr) Hstrip. *)
+    (*                 + apply map_Forall_lookup_2. *)
+    (*                   intros r lw' Hr. *)
+    (*                   destruct (decide (r = src)); subst. *)
+    (*                   rewrite lookup_delete in Hr; congruence. *)
+    (*                   rewrite lookup_delete_ne in Hr; eauto. *)
+    (*                   apply Hunique in Hlr_src. destruct Hlr_src as [Hunique_reg _]. *)
+    (*                   rewrite /unique_in_registersL in Hunique_reg. *)
+    (*                   eapply map_Forall_lookup_1 in Hunique_reg ; eauto. *)
+    (*                   rewrite decide_False in Hunique_reg; auto. *)
+    (*                   eapply map_Forall_lookup_1 in Hcur_reg ; eauto. *)
+    (*                   eapply update_cur_version_notin_is_cur_word ; eauto. *)
+    (*                   Unshelve. all: auto. *)
+    (*             Qed. *)
+
+    (*             eapply update_cur_version_reg_phys_log_cor_updates_src_s with *)
+    (*               (phm := mem). *)
+    (*             Lemma update_cur_version_region_update_lscap *)
+    (*               (lm lm' : LMem) (cur_map cur_map' : VMap) *)
+    (*               (o : OType) (p : Perm) (b e a : Addr) (v : Version) : *)
+    (*               update_cur_version_region lm cur_map (finz.seq_between b e) = Some (lm', cur_map') -> *)
+    (*               is_cur_word (LSealedCap o p b e a v) cur_map -> *)
+    (*               is_cur_word (LSealedCap o p b e a (v + 1)) cur_map'. *)
+    (*             Proof. *)
+    (*               move=> Hupd Hcur. *)
+    (*               rewrite -/(update_version_lword (LSealedCap o p b e a v)). *)
+    (*               eapply update_cur_version_word_region_update_lword; cbn ; eauto. *)
+    (*             Qed. *)
+
+    (*             eapply update_cur_version_region_update_lscap; eauto. *)
+    (*             eapply lreg_read_iscur; eauto. *)
+    (*             2: by rewrite lookup_insert_ne // lookup_insert_ne //. *)
+    (*             2: { *)
+    (*               eapply unique_in_machineL_insert_reg; eauto ; try by simplify_map_eq. *)
+    (*               Lemma not_overlap_word_leaL *)
+    (*                 (lw : LWord) (p : Perm) (b e a a' : Addr) (v : Version) : *)
+    (*                 ¬ overlap_wordL lw (LCap p b e a v) -> *)
+    (*                 ¬ overlap_wordL lw (LCap p b e a' v). *)
+    (*               Proof. *)
+    (*                 move=> Hno_overlap Hoverlap. *)
+    (*                 apply Hno_overlap. *)
+    (*                 rewrite /overlap_wordL ; rewrite /overlap_wordL in Hoverlap *)
+    (*                 ; cbn in *; done. *)
+    (*               Qed. *)
+
+    (*               eapply not_overlap_word_leaL with (a' := a1); eauto. *)
+    (*               eapply (unique_in_machineL_not_overlap_word _ _ src PC); eauto. *)
+
+    (*               eapply unique_in_machineL_insert_reg; eauto *)
+    (*               ; try by simplify_map_eq. *)
+    (*             } *)
+    (*             split; eauto. *)
+    (*             eapply lreg_insert_respects_corresponds; eauto. *)
+    (*             eapply lreg_insert_respects_corresponds; eauto. *)
+    (*             by cbn. *)
+    (*             apply is_cur_word_lea with (a := a1). *)
+    (*             eapply lreg_read_iscur; eauto. *)
+    (*             eauto. *)
+    (*           } *)
+    (*           { *)
+    (*             Lemma mem_phys_log_update_s *)
+    (*               (reg : Reg) (mem : Mem) *)
+    (*               (lr : LReg) (lm lm' : LMem) (cur_map cur_map' : VMap) *)
+    (*               (src : RegName) (o : OType) (p : Perm) (b e a : Addr) (v : Version) : *)
+    (*               (* necessary for lreg_res_iscur *) *)
+    (*               reg_phys_log_corresponds reg lr cur_map -> *)
+    (*               (* necessary for unique_in_machine_no_accessL *) *)
+    (*               lr !! src = Some (LSealedCap o p b e a v) -> *)
+    (*               unique_in_machineL lm lr src (LSealedCap o p b e a v) -> *)
+
+    (*               (* necessary for update_cur_version... *) *)
+    (*               NoDup (finz.seq_between b e) -> *)
+    (*               update_cur_version_region lm cur_map (finz.seq_between b e) *)
+    (*               = Some (lm', cur_map') -> *)
+    (*               mem_phys_log_corresponds mem lm cur_map -> *)
+    (*               mem_phys_log_corresponds mem lm' cur_map'. *)
+    (*             Proof. *)
+    (*               intros. *)
+    (*               eapply update_cur_version_region_preserves_mem_phyc_cor; eauto. *)
+
+    (*               Lemma unique_in_machine_no_accessL_s *)
+    (*                 (phm : Mem) (lm : LMem) (lr : LReg) (cur_map : VMap) (src : RegName) *)
+    (*                 (o : OType) (p : Perm) (b e a : Addr) ( v : Version ) : *)
+    (*                 mem_phys_log_corresponds phm lm cur_map -> *)
+    (*                 lr !! src = Some (LSealedCap o p b e a v) -> *)
+    (*                 is_cur_word (LSealedCap o p b e a v) cur_map -> *)
+    (*                 unique_in_machineL lm lr src (LSealedCap o p b e a v) -> *)
+    (*                 Forall *)
+    (*                   (λ a' : Addr, lmem_not_access_addrL lm cur_map a') *)
+    (*                   (finz.seq_between b e). *)
+    (*               Proof. *)
+    (*                 move=> Hmem_inv Hlr_src His_cur Hunique. *)
+    (*                 apply Forall_forall. *)
+    (*                 move=> a' Ha'. *)
+    (*                 pose proof (is_cur_word_lea cur_map p b e a a' v His_cur) as His_cur'. *)
+    (*                 assert (Hcur_a': is_cur_addr (a',v) cur_map). *)
+    (*                 { eapply (cur_lword_cur_addr _ _ b e) ; eauto; cycle 1. *)
+    (*                   apply withinBounds_true_iff. *)
+    (*                   apply elem_of_finz_seq_between in Ha'. *)
+    (*                   solve_addr. *)
+    (*                   rewrite /is_lword_version //=. *)
+    (*                 } *)
+
+    (*                 rewrite /unique_in_machineL in Hunique. *)
+    (*                 specialize (Hunique Hlr_src). *)
+    (*                 destruct Hunique as [Hunique_reg Hunique_mem]. *)
+    (*                 eapply map_Forall_impl ; first eapply Hunique_mem. *)
+    (*                 move=> [a0 v0] lw0 Hlast_v Hcur_v0. *)
+    (*                 eapply no_overlap_word_no_access_addrL ; eauto. *)
+    (*                 eapply Hlast_v. *)
+    (*                 eapply mem_phys_log_cur_addr_last_version_1; eauto. *)
+    (*                 Unshelve. all: auto. *)
+    (*               Qed. *)
+
+    (*               eapply unique_in_machine_no_accessL_s ; eauto. *)
+    (*               eapply lreg_read_iscur; eauto. *)
+    (*             Qed. *)
+
+    (*             eapply mem_phys_log_update_s ; eauto. } *)
+
+    (*         * (* src = dst *) *)
+    (*           iMod ((gen_heap_update_inSepM _ _ dst (LInt 1)) with "Hr Hmap") *)
+    (*             as "[Hr Hmap]"; eauto. *)
+    (*           iMod ((gen_heap_update_inSepM _ _ PC (LCap p1 b1 e1 a_pc1 v1)) with "Hr Hmap") *)
+    (*             as "[Hr Hmap]"; eauto ; first by simplify_map_eq. *)
+
+    (*           iFrame; iModIntro ; iSplitR "Hφ Hmap Hmem" *)
+    (*           ; [| iApply "Hφ" ; iFrame; iPureIntro; econstructor; eauto]. *)
+    (*           2: { rewrite insert_insert in H'lregs'. *)
+    (*                rewrite insert_insert. done. *)
+    (*           } *)
+    (*           iExists _, lm', cur_map'; iFrame; auto *)
+    (*           ; iPureIntro; econstructor; eauto *)
+    (*           ; destruct HLinv as [Hreg_inv Hmem_inv] *)
+    (*           ; cbn in *. *)
+    (*           { *)
+    (*             rewrite (insert_commute _ _ dst) // (insert_commute _ _ dst) //. *)
+    (*             assert (HPC' := lookup_weaken _ _ _ _ HPC'' Hregs). *)
+
+    (*             eapply update_cur_version_reg_phys_log_cor_updates_src_s *)
+    (*               with (phm := mem) ; eauto. *)
+    (*             done. *)
+    (*             2: by rewrite lookup_insert_ne // lookup_insert_ne //. *)
+    (*             2: { *)
+    (*               eapply unique_in_machineL_insert_reg; eauto ; try by simplify_map_eq. *)
+    (*               eapply not_overlap_word_leaL with (a' := a1); eauto. *)
+    (*               eapply (unique_in_machineL_not_overlap_word _ lr dst); eauto. *)
+    (*             } *)
+    (*             split; eauto. *)
+    (*             eapply lreg_insert_respects_corresponds; eauto. *)
+    (*             apply is_cur_word_lea with (a := a1). *)
+    (*             eapply lreg_read_iscur; eauto. *)
+    (*           } *)
+    (*           { eapply mem_phys_log_update_s ; eauto. } *)
+
+    (*     - (* sweep = false *) *)
+
+    (*       destruct (incrementLPC (<[ dst := LInt 0 ]> lregs)) *)
+    (*         as  [ lregs' |] eqn:Hlregs' *)
+    (*       ; pose proof Hlregs' as H'lregs' *)
+    (*       ; cycle 1. *)
+    (*       {  (* Failure: the PC could not be incremented correctly *) *)
+    (*         apply incrementLPC_fail_updatePC with (m:=mem) (etbl:=etable) (ecur:=enumcur) in Hlregs'. *)
+    (*         eapply updatePC_fail_incl with (m':=mem) (etbl':=etable) (ecur':=enumcur) in Hlregs'. *)
+    (*         2: { *)
+    (*           rewrite /lreg_strip lookup_fmap. *)
+    (*           apply fmap_is_Some. *)
+    (*           destruct (decide (dst = PC)) ; simplify_map_eq; auto. *)
+    (*         } *)
+    (*         2: apply map_fmap_mono ; apply insert_mono ; eauto. *)
+    (*         replace ((λ lw : LWord, lword_get_word lw) <$> (<[dst:=LInt 0]> lr)) *)
+    (*           with (<[dst:= WInt 0]> reg) *)
+    (*           in Hlregs' *)
+    (*         ; cycle 1. *)
+    (*         { destruct HLinv as [ [Hstrips Hcurreg] _]. *)
+    (*           rewrite -Hstrips !fmap_insert -/(lreg_strip lr) //=. *)
+    (*         } *)
+
+    (*         rewrite Hlregs' in Hstep. inversion Hstep. *)
+    (*         iSplitR "Hφ Hmap Hmem" *)
+    (*         ; [ iExists lr, lm, cur_map; iFrame; auto *)
+    (*           | iApply "Hφ" ; iFrame ; iFailCore IsUnique_fail_invalid_PC_false *)
+    (*           ]. *)
+    (*       } *)
+
+    (*       (* PC has been incremented correctly *) *)
+    (*       rewrite /update_reg /= in Hstep. *)
+    (*       eapply (incrementLPC_success_updatePC _ mem etable enumcur) in Hlregs' *)
+    (*           as (p1 & b1 & e1 & a1 & a_pc1 & v1 & HPC'' & Ha_pc' & HuPC & ->) *)
+    (*       ; simplify_map_eq. *)
+    (*       assert (dst <> PC) as Hdst by (intro ; simplify_map_eq). *)
+    (*       eapply updatePC_success_incl with (m':=mem) (etbl':=etable) (ecur':=enumcur) in HuPC. *)
+    (*       2: apply map_fmap_mono ; apply insert_mono ; eauto. *)
+    (*       replace ((λ lw, lword_get_word lw) <$> <[dst:=LInt 0]> lr) *)
+    (*         with (<[dst:=WInt 0]> reg) in HuPC. *)
+    (*       2: { destruct HLinv as [ [Hstrips Hcurreg] _] *)
+    (*            ; rewrite -Hstrips !fmap_insert -/(lreg_strip lr) //=. *)
+    (*       } *)
+    (*       rewrite HuPC in Hstep; clear HuPC. *)
+    (*       inversion Hstep; clear Hstep ; simplify_map_eq. *)
+
+    (*       iMod ((gen_heap_update_inSepM _ _ dst ) with "Hr Hmap") as "[Hr Hmap]"; eauto. *)
+    (*       iMod ((gen_heap_update_inSepM _ _ PC ) with "Hr Hmap") as "[Hr Hmap]"; eauto *)
+    (*       ; first by simplify_map_eq. *)
+
+    (*       iFrame; iModIntro ; iSplitR "Hφ Hmap Hmem" *)
+    (*       ; [| iApply "Hφ" ; iFrame; iPureIntro; eapply IsUnique_success_false ; eauto]. *)
+
+    (*       iExists _, lm, cur_map; iFrame; auto *)
+    (*       ; iPureIntro; econstructor; eauto *)
+    (*       ; destruct HLinv as [ [Hstrips Hcur_reg] [Hdom Hroot] ] *)
+    (*       ; cbn in * *)
+    (*       ; [|split;eauto] *)
+    (*       . *)
+    (*       split; first by rewrite -Hstrips /lreg_strip !fmap_insert /=. *)
+    (*       apply map_Forall_insert_2 ; [|by apply map_Forall_insert_2; cbn]. *)
+    (*       rewrite HPC in HPC'' ; simplify_eq. *)
+    (*       eapply is_cur_word_cap_change; eauto. *)
+    (*       Unshelve. all: eauto. *)
+    (*   } *)
+  Admitted.
 
   (* Because I don't know the whole content of the memory (only a local view),
      any sucessful IsUnique wp-rule can have 2 outcomes:
@@ -658,261 +954,261 @@ Section cap_lang_rules.
     the entire footprint of the registers/memory.
    *)
 
-  Lemma update_version_word_region_cons_no_access_gen
-    (lm lm' : LMem) (a : Addr) (la : list Addr) (v v' : Version) (lw : LWord):
-    NoDup la ->
-    a ∉ la ->
-    foldr
-      (λ (a : Addr) (upd_opt : option LMem),
-        upd_opt ≫= (λ lmem', update_version_addr lmem' a v')
-      )
-      (Some (<[(a,v):=lw]> lm))
-      la = Some lm'
-    -> ∃ lm'',
-        foldr
-          (λ (a : Addr) (upd_opt : option LMem),
-            upd_opt ≫= (λ lmem', update_version_addr lmem' a v')
-          )
-          (Some lm) la = Some lm''
-        ∧ lm' = <[(a,v):=lw]> lm''.
-  Proof.
-    move: lm lm' a v v' lw.
-    induction la as [|a la Hla]; intros ? ? a' * HNoDup Ha'_notin_la Hupd
-    ; cbn in * ; simplify_eq.
-    - eexists ; split ; eauto.
-    - apply NoDup_cons in HNoDup
-      ; destruct HNoDup as [Ha_notin_la HNoDup].
+  (* Lemma update_version_word_region_cons_no_access_gen *)
+  (*   (lm lm' : LMem) (a : Addr) (la : list Addr) (v v' : Version) (lw : LWord): *)
+  (*   NoDup la -> *)
+  (*   a ∉ la -> *)
+  (*   foldr *)
+  (*     (λ (a : Addr) (upd_opt : option LMem), *)
+  (*       upd_opt ≫= (λ lmem', update_version_addr lmem' a v') *)
+  (*     ) *)
+  (*     (Some (<[(a,v):=lw]> lm)) *)
+  (*     la = Some lm' *)
+  (*   -> ∃ lm'', *)
+  (*       foldr *)
+  (*         (λ (a : Addr) (upd_opt : option LMem), *)
+  (*           upd_opt ≫= (λ lmem', update_version_addr lmem' a v') *)
+  (*         ) *)
+  (*         (Some lm) la = Some lm'' *)
+  (*       ∧ lm' = <[(a,v):=lw]> lm''. *)
+  (* Proof. *)
+  (*   move: lm lm' a v v' lw. *)
+  (*   induction la as [|a la Hla]; intros ? ? a' * HNoDup Ha'_notin_la Hupd *)
+  (*   ; cbn in * ; simplify_eq. *)
+  (*   - eexists ; split ; eauto. *)
+  (*   - apply NoDup_cons in HNoDup *)
+  (*     ; destruct HNoDup as [Ha_notin_la HNoDup]. *)
 
-      apply not_elem_of_cons in Ha'_notin_la
-      ; destruct Ha'_notin_la as [Ha'_neq_a Ha'_notin_la].
+  (*     apply not_elem_of_cons in Ha'_notin_la *)
+  (*     ; destruct Ha'_notin_la as [Ha'_neq_a Ha'_notin_la]. *)
 
-      apply bind_Some in Hupd.
-      destruct Hupd as (lm0 & Hupd & Hlm').
-      rewrite /update_version_addr in Hlm'.
-      destruct (lm0 !! (a, v')) as [lw0|] eqn:Heq_lm0
-      ; cbn in * ; simplify_eq.
+  (*     apply bind_Some in Hupd. *)
+  (*     destruct Hupd as (lm0 & Hupd & Hlm'). *)
+  (*     rewrite /update_version_addr in Hlm'. *)
+  (*     destruct (lm0 !! (a, v')) as [lw0|] eqn:Heq_lm0 *)
+  (*     ; cbn in * ; simplify_eq. *)
 
-      eapply Hla in Hupd; eauto.
-      destruct Hupd as (lm0' & Hupd & ->).
-      exists (<[(a, v' + 1):=lw0]> lm0').
-      split; simplify_map_eq ; eauto.
-      + rewrite /update_version_addr.
-        rewrite lookup_insert_ne in Heq_lm0 ; [|intro ; simplify_eq].
-        by rewrite Heq_lm0; cbn.
-      + rewrite insert_commute //. intro ; simplify_eq.
-  Qed.
+  (*     eapply Hla in Hupd; eauto. *)
+  (*     destruct Hupd as (lm0' & Hupd & ->). *)
+  (*     exists (<[(a, v' + 1):=lw0]> lm0'). *)
+  (*     split; simplify_map_eq ; eauto. *)
+  (*     + rewrite /update_version_addr. *)
+  (*       rewrite lookup_insert_ne in Heq_lm0 ; [|intro ; simplify_eq]. *)
+  (*       by rewrite Heq_lm0; cbn. *)
+  (*     + rewrite insert_commute //. intro ; simplify_eq. *)
+  (* Qed. *)
 
-  Lemma update_version_word_region_cons_no_access
-    (lm lm' : LMem) (la : LAddr) (lw lwsrc : LWord) :
-    update_version_word_region (<[ la := lw ]> lm) lwsrc = Some lm' ->
-    ¬ (word_access_addrL (laddr_get_addr la) lwsrc) ->
-    exists lm'', (update_version_word_region lm lwsrc) = Some lm''
-            /\ lm' = <[ la := lw ]> lm''.
-  Proof.
-    intros Hupd Hno_access.
-    destruct la as [a' v'].
-    rewrite /update_version_word_region in Hupd.
-    destruct_lword lwsrc ; try (by simplify_map_eq ; eexists ; eauto).
-    all: eapply update_version_word_region_cons_no_access_gen in Hupd;
-      [| apply finz_seq_between_NoDup
-      | cbn in *; intros Hcontra ; apply elem_of_finz_seq_between in Hcontra; done].
-    all: destruct Hupd as (lm'' & Hupd & ->).
-    all: exists lm''; split ; eauto.
-  Qed.
+  (* Lemma update_version_word_region_cons_no_access *)
+  (*   (lm lm' : LMem) (la : LAddr) (lw lwsrc : LWord) : *)
+  (*   update_version_word_region (<[ la := lw ]> lm) lwsrc = Some lm' -> *)
+  (*   ¬ (word_access_addrL (laddr_get_addr la) lwsrc) -> *)
+  (*   exists lm'', (update_version_word_region lm lwsrc) = Some lm'' *)
+  (*           /\ lm' = <[ la := lw ]> lm''. *)
+  (* Proof. *)
+  (*   intros Hupd Hno_access. *)
+  (*   destruct la as [a' v']. *)
+  (*   rewrite /update_version_word_region in Hupd. *)
+  (*   destruct_lword lwsrc ; try (by simplify_map_eq ; eexists ; eauto). *)
+  (*   all: eapply update_version_word_region_cons_no_access_gen in Hupd; *)
+  (*     [| apply finz_seq_between_NoDup *)
+  (*     | cbn in *; intros Hcontra ; apply elem_of_finz_seq_between in Hcontra; done]. *)
+  (*   all: destruct Hupd as (lm'' & Hupd & ->). *)
+  (*   all: exists lm''; split ; eauto. *)
+  (* Qed. *)
 
-  Lemma update_version_word_preserves_lword
-    (lm lmem : LMem) (la : list Addr) (a : Addr) (v : Version) (lw lw' : LWord)
-    :
-    foldr
-      (λ (a : Addr) (upd_opt : option LMem),
-        upd_opt ≫= (λ lmem', update_version_addr lmem' a v))
-      (Some (<[(a, v):= lw]> lmem)) la =
-      Some lm ->
-    lm !! (a, v) = Some lw' ->
-    lw = lw'.
-  Proof.
-    move: lm lmem a v lw lw'.
-    induction la as [| a la Hla] ; intros * Hupd Hlookup
-    ; cbn in * ; simplify_map_eq ; first done.
-    apply bind_Some in Hupd.
-    destruct Hupd as (lm0 & Hupd & Hlm).
-    rewrite /update_version_addr in Hlm.
-    destruct (lm0 !! (a,v)) as [lw0|] eqn:Heq_lm0; cbn in * ; simplify_eq.
+  (* Lemma update_version_word_preserves_lword *)
+  (*   (lm lmem : LMem) (la : list Addr) (a : Addr) (v : Version) (lw lw' : LWord) *)
+  (*   : *)
+  (*   foldr *)
+  (*     (λ (a : Addr) (upd_opt : option LMem), *)
+  (*       upd_opt ≫= (λ lmem', update_version_addr lmem' a v)) *)
+  (*     (Some (<[(a, v):= lw]> lmem)) la = *)
+  (*     Some lm -> *)
+  (*   lm !! (a, v) = Some lw' -> *)
+  (*   lw = lw'. *)
+  (* Proof. *)
+  (*   move: lm lmem a v lw lw'. *)
+  (*   induction la as [| a la Hla] ; intros * Hupd Hlookup *)
+  (*   ; cbn in * ; simplify_map_eq ; first done. *)
+  (*   apply bind_Some in Hupd. *)
+  (*   destruct Hupd as (lm0 & Hupd & Hlm). *)
+  (*   rewrite /update_version_addr in Hlm. *)
+  (*   destruct (lm0 !! (a,v)) as [lw0|] eqn:Heq_lm0; cbn in * ; simplify_eq. *)
 
-    eapply Hla in Hupd; eauto.
-    rewrite lookup_insert_ne // in Hlookup.
-    intro ; simplify_eq; lia.
-  Qed.
+  (*   eapply Hla in Hupd; eauto. *)
+  (*   rewrite lookup_insert_ne // in Hlookup. *)
+  (*   intro ; simplify_eq; lia. *)
+  (* Qed. *)
 
-  Lemma update_version_word_region_insert
-    (lm lmem : LMem) (la : list Addr) (a : Addr) (v : Version) (w : LWord) :
-    a ∉ la ->
-    foldr
-      (λ (a : Addr) (upd_opt : option LMem),
-        upd_opt ≫= (λ lmem', update_version_addr lmem' a v))
-      (Some (<[(a, v):=w]> lmem))
-      la = Some lm ->
-    exists lm',
-      foldr
-        (λ (a : Addr) (upd_opt : option LMem),
-          upd_opt ≫= (λ lmem', update_version_addr lmem' a v))
-        (Some lmem)
-        la = Some lm'
-      /\ lm = <[(a, v):=w]> lm'.
-  Proof.
-    move: lm lmem a v w.
-    induction la as [|a la Hla] ; intros * Hnot_in Hupd; cbn in *
-    ; simplify_map_eq; first set_solver.
+  (* Lemma update_version_word_region_insert *)
+  (*   (lm lmem : LMem) (la : list Addr) (a : Addr) (v : Version) (w : LWord) : *)
+  (*   a ∉ la -> *)
+  (*   foldr *)
+  (*     (λ (a : Addr) (upd_opt : option LMem), *)
+  (*       upd_opt ≫= (λ lmem', update_version_addr lmem' a v)) *)
+  (*     (Some (<[(a, v):=w]> lmem)) *)
+  (*     la = Some lm -> *)
+  (*   exists lm', *)
+  (*     foldr *)
+  (*       (λ (a : Addr) (upd_opt : option LMem), *)
+  (*         upd_opt ≫= (λ lmem', update_version_addr lmem' a v)) *)
+  (*       (Some lmem) *)
+  (*       la = Some lm' *)
+  (*     /\ lm = <[(a, v):=w]> lm'. *)
+  (* Proof. *)
+  (*   move: lm lmem a v w. *)
+  (*   induction la as [|a la Hla] ; intros * Hnot_in Hupd; cbn in * *)
+  (*   ; simplify_map_eq; first set_solver. *)
 
-    apply not_elem_of_cons in Hnot_in; destruct Hnot_in as [Hneq Hnot_in].
+  (*   apply not_elem_of_cons in Hnot_in; destruct Hnot_in as [Hneq Hnot_in]. *)
 
-    apply bind_Some in Hupd.
-    destruct Hupd as ( lm' & Hupd & Hlm ).
-    rewrite /update_version_addr in Hlm.
-    destruct (lm' !! (a, v)) as [lw|] eqn:Heq_lm; cbn in * ; simplify_eq.
-    eapply Hla in Hupd; auto.
-    destruct Hupd as ( lm0 & Hupd & -> ).
+  (*   apply bind_Some in Hupd. *)
+  (*   destruct Hupd as ( lm' & Hupd & Hlm ). *)
+  (*   rewrite /update_version_addr in Hlm. *)
+  (*   destruct (lm' !! (a, v)) as [lw|] eqn:Heq_lm; cbn in * ; simplify_eq. *)
+  (*   eapply Hla in Hupd; auto. *)
+  (*   destruct Hupd as ( lm0 & Hupd & -> ). *)
 
-    exists (<[(a, v + 1):=lw]> lm0).
-    split ; cycle 1.
-    rewrite insert_commute //=; intro ; simplify_eq.
+  (*   exists (<[(a, v + 1):=lw]> lm0). *)
+  (*   split ; cycle 1. *)
+  (*   rewrite insert_commute //=; intro ; simplify_eq. *)
 
-    apply bind_Some.
-    exists (<[(a, v):=lw]> lm0).
-    rewrite lookup_insert_ne in Heq_lm ; [| intro ; simplify_eq ; lia].
-    rewrite /update_version_addr.
-    split; cycle 1; simplify_map_eq ; rewrite (insert_id _ (a,v)); auto.
-  Qed.
+  (*   apply bind_Some. *)
+  (*   exists (<[(a, v):=lw]> lm0). *)
+  (*   rewrite lookup_insert_ne in Heq_lm ; [| intro ; simplify_eq ; lia]. *)
+  (*   rewrite /update_version_addr. *)
+  (*   split; cycle 1; simplify_map_eq ; rewrite (insert_id _ (a,v)); auto. *)
+  (* Qed. *)
 
-  Lemma update_version_word_region_access_region_gen
-    (lm : LMem) (lws : list LWord) (v : Version) (la : list Addr) :
-    NoDup la ->
-    length lws = length la ->
-    foldr
-      (λ (a : Addr) (upd_opt : option LMem),
-        upd_opt ≫= (λ lmem', update_version_addr lmem' a v))
-      (Some (list_to_map (zip (map (λ a : Addr, (a, v)) la) lws)))
-      la = Some lm ->
-    lm = (list_to_map
-            ((zip (map (λ a : Addr, (a, v+1)) la) lws)
-               ++ (zip (map (λ a : Addr, (a, v)) la) lws))
-         ).
-  Proof.
-    move: lm lws v.
-    induction la as [| a la Hla]; intros * HNoDup Hlen_eq Hupd
-    ; cbn in * ; simplify_map_eq; first done.
-    apply NoDup_cons in HNoDup; destruct HNoDup as [Ha_notin_la HNoDup].
-    destruct lws; cbn in * ; try congruence.
-    injection Hlen_eq; clear Hlen_eq ; intro Hlen_eq.
+  (* Lemma update_version_word_region_access_region_gen *)
+  (*   (lm : LMem) (lws : list LWord) (v : Version) (la : list Addr) : *)
+  (*   NoDup la -> *)
+  (*   length lws = length la -> *)
+  (*   foldr *)
+  (*     (λ (a : Addr) (upd_opt : option LMem), *)
+  (*       upd_opt ≫= (λ lmem', update_version_addr lmem' a v)) *)
+  (*     (Some (list_to_map (zip (map (λ a : Addr, (a, v)) la) lws))) *)
+  (*     la = Some lm -> *)
+  (*   lm = (list_to_map *)
+  (*           ((zip (map (λ a : Addr, (a, v+1)) la) lws) *)
+  (*              ++ (zip (map (λ a : Addr, (a, v)) la) lws)) *)
+  (*        ). *)
+  (* Proof. *)
+  (*   move: lm lws v. *)
+  (*   induction la as [| a la Hla]; intros * HNoDup Hlen_eq Hupd *)
+  (*   ; cbn in * ; simplify_map_eq; first done. *)
+  (*   apply NoDup_cons in HNoDup; destruct HNoDup as [Ha_notin_la HNoDup]. *)
+  (*   destruct lws; cbn in * ; try congruence. *)
+  (*   injection Hlen_eq; clear Hlen_eq ; intro Hlen_eq. *)
 
-    apply bind_Some in Hupd.
-    destruct Hupd as ( lm' & Hupd & Hlm ).
-    rewrite /update_version_addr in Hlm.
-    destruct (lm' !! (a, v)) as [lw|] eqn:Heq_lm; cbn in * ; simplify_eq.
+  (*   apply bind_Some in Hupd. *)
+  (*   destruct Hupd as ( lm' & Hupd & Hlm ). *)
+  (*   rewrite /update_version_addr in Hlm. *)
+  (*   destruct (lm' !! (a, v)) as [lw|] eqn:Heq_lm; cbn in * ; simplify_eq. *)
 
-    replace l with lw by (symmetry ; eapply update_version_word_preserves_lword; eauto).
-    apply update_version_word_region_insert in Hupd; auto.
-    destruct Hupd as (lm0 & Hupd & ->).
-    simplify_map_eq.
+  (*   replace l with lw by (symmetry ; eapply update_version_word_preserves_lword; eauto). *)
+  (*   apply update_version_word_region_insert in Hupd; auto. *)
+  (*   destruct Hupd as (lm0 & Hupd & ->). *)
+  (*   simplify_map_eq. *)
 
-    eapply Hla in Hupd; eauto.
-    simplify_map_eq.
-    rewrite !list_to_map_app.
-    rewrite list_to_map_cons.
-    rewrite insert_union_r; first done.
+  (*   eapply Hla in Hupd; eauto. *)
+  (*   simplify_map_eq. *)
+  (*   rewrite !list_to_map_app. *)
+  (*   rewrite list_to_map_cons. *)
+  (*   rewrite insert_union_r; first done. *)
 
-    apply not_elem_of_list_to_map_1 ; cbn.
-    rewrite fst_zip; [|rewrite map_length; lia].
-    intro Hcontra.
-    apply elem_of_list_fmap in Hcontra.
-    destruct Hcontra as (a0 & Hcontra & _).
-    simplify_eq; lia.
-  Qed.
+  (*   apply not_elem_of_list_to_map_1 ; cbn. *)
+  (*   rewrite fst_zip; [|rewrite map_length; lia]. *)
+  (*   intro Hcontra. *)
+  (*   apply elem_of_list_fmap in Hcontra. *)
+  (*   destruct Hcontra as (a0 & Hcontra & _). *)
+  (*   simplify_eq; lia. *)
+  (* Qed. *)
 
-  Lemma update_version_word_region_access_region
-    (lm lm' : LMem) (lwsrc : LWord) (lws : list LWord)
-    (p : Perm) (b e a : Addr) (v : Version) :
-    length lws = length (finz.seq_between b e) ->
-    get_lcap lwsrc = Some (LSCap p b e a v) ->
-    update_version_word_region
-      (list_to_map (zip (map (λ a : Addr, (a, v)) (finz.seq_between b e)) lws))
-      lwsrc = Some lm' ->
-    lm' =
-      (list_to_map
-         ((zip (map (λ a : Addr, (a, v+1)) (finz.seq_between b e)) lws)
-         ++ (zip (map (λ a : Addr, (a, v)) (finz.seq_between b e)) lws))).
-  Proof.
-    intros Hlen_lws Hlwsrc Hupd.
-    rewrite /update_version_word_region in Hupd.
-    destruct_lword lwsrc ; cbn in * ; simplify_eq.
-    all: eapply update_version_word_region_access_region_gen; eauto
-    ; apply finz_seq_between_NoDup.
-  Qed.
+  (* Lemma update_version_word_region_access_region *)
+  (*   (lm lm' : LMem) (lwsrc : LWord) (lws : list LWord) *)
+  (*   (p : Perm) (b e a : Addr) (v : Version) : *)
+  (*   length lws = length (finz.seq_between b e) -> *)
+  (*   get_lcap lwsrc = Some (LSCap p b e a v) -> *)
+  (*   update_version_word_region *)
+  (*     (list_to_map (zip (map (λ a : Addr, (a, v)) (finz.seq_between b e)) lws)) *)
+  (*     lwsrc = Some lm' -> *)
+  (*   lm' = *)
+  (*     (list_to_map *)
+  (*        ((zip (map (λ a : Addr, (a, v+1)) (finz.seq_between b e)) lws) *)
+  (*        ++ (zip (map (λ a : Addr, (a, v)) (finz.seq_between b e)) lws))). *)
+  (* Proof. *)
+  (*   intros Hlen_lws Hlwsrc Hupd. *)
+  (*   rewrite /update_version_word_region in Hupd. *)
+  (*   destruct_lword lwsrc ; cbn in * ; simplify_eq. *)
+  (*   all: eapply update_version_word_region_access_region_gen; eauto *)
+  (*   ; apply finz_seq_between_NoDup. *)
+  (* Qed. *)
 
-  (* TODO better name because it means nothing *)
-  Lemma logical_region_reachable
-    (la : list Addr)
-    (pc_a a : Addr) (lws : list LWord)
-    (pc_v v : Version) (lw : LWord) :
-    NoDup la ->
-    pc_a ∉ la ->
-    length lws = length la ->
-    a ∈ la ->
-    ∃ lw0,
-      (<[(pc_a, pc_v):=lw]>
-         (list_to_map (zip (map (λ a0 : Addr, (a0, v)) la) lws)) : LMem)
-        !! (a, v) = Some lw0.
-  Proof.
-    move: pc_a a lws pc_v v lw.
-    induction la as [|a la Hla]
-    ; intros * HNoDup Hpca_notin_la Hlen Ha_in_la
-    ; cbn in * ; simplify_map_eq ; first set_solver.
+  (* (* TODO better name because it means nothing *) *)
+  (* Lemma logical_region_reachable *)
+  (*   (la : list Addr) *)
+  (*   (pc_a a : Addr) (lws : list LWord) *)
+  (*   (pc_v v : Version) (lw : LWord) : *)
+  (*   NoDup la -> *)
+  (*   pc_a ∉ la -> *)
+  (*   length lws = length la -> *)
+  (*   a ∈ la -> *)
+  (*   ∃ lw0, *)
+  (*     (<[(pc_a, pc_v):=lw]> *)
+  (*        (list_to_map (zip (map (λ a0 : Addr, (a0, v)) la) lws)) : LMem) *)
+  (*       !! (a, v) = Some lw0. *)
+  (* Proof. *)
+  (*   move: pc_a a lws pc_v v lw. *)
+  (*   induction la as [|a la Hla] *)
+  (*   ; intros * HNoDup Hpca_notin_la Hlen Ha_in_la *)
+  (*   ; cbn in * ; simplify_map_eq ; first set_solver. *)
 
-    apply not_elem_of_cons in Hpca_notin_la.
-    destruct Hpca_notin_la as [Hpca_neq_a Hpca_notin_la].
-    destruct lws; cbn in * ; try congruence.
-    injection Hlen; clear Hlen ; intro Hlen.
-    apply NoDup_cons in HNoDup.
-    destruct HNoDup as [Ha_notin_la HNoDup].
+  (*   apply not_elem_of_cons in Hpca_notin_la. *)
+  (*   destruct Hpca_notin_la as [Hpca_neq_a Hpca_notin_la]. *)
+  (*   destruct lws; cbn in * ; try congruence. *)
+  (*   injection Hlen; clear Hlen ; intro Hlen. *)
+  (*   apply NoDup_cons in HNoDup. *)
+  (*   destruct HNoDup as [Ha_notin_la HNoDup]. *)
 
-    apply elem_of_cons in Ha_in_la.
-    destruct Ha_in_la as [-> | Ha_in_la].
-    - exists l. by rewrite lookup_insert_ne; [| intro ; simplify_eq] ; simplify_map_eq.
-    - pose proof (Hla _ _ _ pc_v v lw HNoDup Hpca_notin_la Hlen Ha_in_la) as IH.
-      destruct IH as (lw0 & IH).
-      exists lw0.
-      rewrite insert_commute; [| intro ; simplify_eq].
-      rewrite lookup_insert_ne ; [|intro ; simplify_eq].
-      done.
-  Qed.
+  (*   apply elem_of_cons in Ha_in_la. *)
+  (*   destruct Ha_in_la as [-> | Ha_in_la]. *)
+  (*   - exists l. by rewrite lookup_insert_ne; [| intro ; simplify_eq] ; simplify_map_eq. *)
+  (*   - pose proof (Hla _ _ _ pc_v v lw HNoDup Hpca_notin_la Hlen Ha_in_la) as IH. *)
+  (*     destruct IH as (lw0 & IH). *)
+  (*     exists lw0. *)
+  (*     rewrite insert_commute; [| intro ; simplify_eq]. *)
+  (*     rewrite lookup_insert_ne ; [|intro ; simplify_eq]. *)
+  (*     done. *)
+  (* Qed. *)
 
-  (* TODO move region.v *)
-  Lemma NoDup_logical_region (b e : Addr) (v : Version) :
-    NoDup (map (λ a0 : Addr, (a0, v)) (finz.seq_between b e)).
-  Proof.
-    apply NoDup_fmap.
-    { by intros x y Heq ; simplify_eq. }
-    { apply finz_seq_between_NoDup. }
-  Qed.
+  (* (* TODO move region.v *) *)
+  (* Lemma NoDup_logical_region (b e : Addr) (v : Version) : *)
+  (*   NoDup (map (λ a0 : Addr, (a0, v)) (finz.seq_between b e)). *)
+  (* Proof. *)
+  (*   apply NoDup_fmap. *)
+  (*   { by intros x y Heq ; simplify_eq. } *)
+  (*   { apply finz_seq_between_NoDup. } *)
+  (* Qed. *)
 
-  (* TODO move region.v *)
-  Lemma update_logical_memory_region_disjoint
-    (la : list Addr) (v : Version) (lws : list LWord):
-    length la = length lws ->
-    (list_to_map (zip (map (λ a : Addr, (a, v + 1)) la) lws) : LMem)
-      ##ₘ list_to_map (zip (map (λ a : Addr, (a, v)) la) lws).
-  Proof.
-    intros Hlen.
-    apply map_disjoint_list_to_map_zip_l ; [rewrite map_length; lia|].
-    apply Forall_forall.
-    intros a Ha.
-    apply not_elem_of_list_to_map.
-    rewrite fst_zip; [|rewrite map_length; lia].
-    intros Ha'.
-    apply elem_of_list_fmap_2 in Ha, Ha'.
-    destruct Ha as (? & Ha & ?).
-    destruct Ha' as (? & Ha' & ?). simplify_eq; lia.
-  Qed.
+  (* (* TODO move region.v *) *)
+  (* Lemma update_logical_memory_region_disjoint *)
+  (*   (la : list Addr) (v : Version) (lws : list LWord): *)
+  (*   length la = length lws -> *)
+  (*   (list_to_map (zip (map (λ a : Addr, (a, v + 1)) la) lws) : LMem) *)
+  (*     ##ₘ list_to_map (zip (map (λ a : Addr, (a, v)) la) lws). *)
+  (* Proof. *)
+  (*   intros Hlen. *)
+  (*   apply map_disjoint_list_to_map_zip_l ; [rewrite map_length; lia|]. *)
+  (*   apply Forall_forall. *)
+  (*   intros a Ha. *)
+  (*   apply not_elem_of_list_to_map. *)
+  (*   rewrite fst_zip; [|rewrite map_length; lia]. *)
+  (*   intros Ha'. *)
+  (*   apply elem_of_list_fmap_2 in Ha, Ha'. *)
+  (*   destruct Ha as (? & Ha & ?). *)
+  (*   destruct Ha' as (? & Ha' & ?). simplify_eq; lia. *)
+  (* Qed. *)
 
   Lemma wp_isunique_success
     (Ep : coPset)
@@ -950,99 +1246,100 @@ Section cap_lang_rules.
           ∗ [[ b , e ]] ↦ₐ{ v } [[ lws ]] )
         }}}.
   Proof.
-    iIntros (Hinstr Hvpc Hpca_notin Hpca Hlen_lws φ) "(>HPC & >Hsrc & >Hdst & >Hpc_a & >Hmap) Hφ".
-    iDestruct (map_of_regs_3 with "HPC Hsrc Hdst") as "[Hrmap (%&%&%)]".
-    rewrite /region_mapsto.
-    iDestruct (big_sepL2_cons (λ _ la lw, la ↦ₐ lw)%I (pc_a, pc_v) lw with "[Hpc_a Hmap]")
-      as "Hmmap"; iFrame.
-    iDestruct (big_sepL2_to_big_sepM  with "Hmmap") as "Hmmap".
-    { apply NoDup_cons ; split; [| apply NoDup_logical_region].
-      intro Hcontra.
-      apply elem_of_list_fmap in Hcontra.
-      destruct Hcontra as (? & ? & ?) ; simplify_eq.
-    }
-    iApply (wp_isunique with "[$Hrmap Hmmap]"); eauto ; simplify_map_eq; eauto.
-    { by unfold regs_of; rewrite !dom_insert; set_solver+. }
-    { exists p, b, e, a, v.
-      rewrite /read_reg_inr.
-      split ; simplify_map_eq; eauto.
-      apply Forall_forall.
-      intros a' Ha'.
+  Admitted.
+  (*   iIntros (Hinstr Hvpc Hpca_notin Hpca Hlen_lws φ) "(>HPC & >Hsrc & >Hdst & >Hpc_a & >Hmap) Hφ". *)
+  (*   iDestruct (map_of_regs_3 with "HPC Hsrc Hdst") as "[Hrmap (%&%&%)]". *)
+  (*   rewrite /region_mapsto. *)
+  (*   iDestruct (big_sepL2_cons (λ _ la lw, la ↦ₐ lw)%I (pc_a, pc_v) lw with "[Hpc_a Hmap]") *)
+  (*     as "Hmmap"; iFrame. *)
+  (*   iDestruct (big_sepL2_to_big_sepM  with "Hmmap") as "Hmmap". *)
+  (*   { apply NoDup_cons ; split; [| apply NoDup_logical_region]. *)
+  (*     intro Hcontra. *)
+  (*     apply elem_of_list_fmap in Hcontra. *)
+  (*     destruct Hcontra as (? & ? & ?) ; simplify_eq. *)
+  (*   } *)
+  (*   iApply (wp_isunique with "[$Hrmap Hmmap]"); eauto ; simplify_map_eq; eauto. *)
+  (*   { by unfold regs_of; rewrite !dom_insert; set_solver+. } *)
+  (*   { exists 0%ot, p, b, e, a, v. *)
+  (*     rewrite /read_reg_inr'. *)
+  (*     split ; simplify_map_eq; eauto. *)
+  (*     apply Forall_forall. *)
+  (*     intros a' Ha'. *)
 
-      apply logical_region_reachable; auto.
-      { apply finz_seq_between_NoDup. }
-      { by rewrite finz_seq_between_length. }
-    }
+  (*     apply logical_region_reachable; auto. *)
+  (*     { apply finz_seq_between_NoDup. } *)
+  (*     { by rewrite finz_seq_between_length. } *)
+  (*   } *)
 
-    iNext. iIntros (regs' mem' retv) "(#Hspec & Hmmap & Hrmap)".
-    iDestruct "Hspec" as %Hspec.
-    destruct Hspec as
-      [ ? ? ? ? ? ? Hlwsrc Hlwsrc' Hupd Hincr_PC
-      | ? ? ? ? ? ? Hlwsrc Hlwsrc' Hincr_PC Hmem'
-      | ? ? Hfail]
-    ; cycle 2.
-    - (* Fail : contradiction *)
-      destruct Hfail; try incrementLPC_inv; simplify_map_eq; eauto; solve_addr.
-    - (* Success true *)
-      iApply "Hφ"; iLeft.
+  (*   iNext. iIntros (regs' mem' retv) "(#Hspec & Hmmap & Hrmap)". *)
+  (*   iDestruct "Hspec" as %Hspec. *)
+  (*   destruct Hspec as *)
+  (*     [ ? ? ? ? ? ? Hlwsrc Hlwsrc' Hupd Hincr_PC *)
+  (*     | ? ? ? ? ? ? Hlwsrc Hlwsrc' Hincr_PC Hmem' *)
+  (*     | ? ? Hfail] *)
+  (*   ; cycle 2. *)
+  (*   - (* Fail : contradiction *) *)
+  (*     destruct Hfail; try incrementLPC_inv; simplify_map_eq; eauto; solve_addr. *)
+  (*   - (* Success true *) *)
+  (*     iApply "Hφ"; iLeft. *)
 
-      apply update_version_word_region_cons_no_access in Hupd.
-      2:{ simplify_map_eq; cbn.
-          intro Hcontra.
-          apply elem_of_finz_seq_between in Hcontra. solve_addr.
-      }
-      destruct Hupd as (mem'' & Hupd & ->).
+  (*     apply update_version_word_region_cons_no_access in Hupd. *)
+  (*     2:{ simplify_map_eq; cbn. *)
+  (*         intro Hcontra. *)
+  (*         apply elem_of_finz_seq_between in Hcontra. solve_addr. *)
+  (*     } *)
+  (*     destruct Hupd as (mem'' & Hupd & ->). *)
 
-      eapply update_version_word_region_access_region in Hupd
-      ; eauto; simplify_map_eq ; eauto; [| by rewrite finz_seq_between_length].
+  (*     eapply update_version_word_region_access_region in Hupd *)
+  (*     ; eauto; simplify_map_eq ; eauto; [| by rewrite finz_seq_between_length]. *)
 
 
-      rewrite /incrementLPC in Hincr_PC; simplify_map_eq.
-      iExtractList "Hrmap" [PC; dst; src] as ["HPC"; "Hdst"; "Hsrc"].
-      iClear "Hrmap".
-      iFrame.
-      iDestruct (big_sepM_insert with "Hmmap") as "[Hpc_a Hmmap]".
-      { apply not_elem_of_list_to_map.
-        rewrite fmap_app.
-        do 2 (rewrite fst_zip; [|rewrite map_length finz_seq_between_length; lia]).
-        apply not_elem_of_app.
-        split.
-        all:intros Hcontra.
-        all:apply elem_of_list_fmap_2 in Hcontra.
-        all:destruct Hcontra as (? & Ha & ?); simplify_eq.
-      }
-      iFrame.
-      rewrite list_to_map_app.
-      iDestruct (big_sepM_union with "Hmmap") as "[Hmmap_new Hmmap_old]".
-      { apply update_logical_memory_region_disjoint.
-        by rewrite finz_seq_between_length.
-      }
-      iSplitL "Hmmap_old".
-      + iApply (big_sepM_to_big_sepL2 with "Hmmap_old").
-        { apply NoDup_logical_region. }
-        { by rewrite map_length finz_seq_between_length. }
-      + iApply (big_sepM_to_big_sepL2 with "Hmmap_new").
-        { apply NoDup_logical_region. }
-        { by rewrite map_length finz_seq_between_length. }
+  (*     rewrite /incrementLPC in Hincr_PC; simplify_map_eq. *)
+  (*     iExtractList "Hrmap" [PC; dst; src] as ["HPC"; "Hdst"; "Hsrc"]. *)
+  (*     iClear "Hrmap". *)
+  (*     iFrame. *)
+  (*     iDestruct (big_sepM_insert with "Hmmap") as "[Hpc_a Hmmap]". *)
+  (*     { apply not_elem_of_list_to_map. *)
+  (*       rewrite fmap_app. *)
+  (*       do 2 (rewrite fst_zip; [|rewrite map_length finz_seq_between_length; lia]). *)
+  (*       apply not_elem_of_app. *)
+  (*       split. *)
+  (*       all:intros Hcontra. *)
+  (*       all:apply elem_of_list_fmap_2 in Hcontra. *)
+  (*       all:destruct Hcontra as (? & Ha & ?); simplify_eq. *)
+  (*     } *)
+  (*     iFrame. *)
+  (*     rewrite list_to_map_app. *)
+  (*     iDestruct (big_sepM_union with "Hmmap") as "[Hmmap_new Hmmap_old]". *)
+  (*     { apply update_logical_memory_region_disjoint. *)
+  (*       by rewrite finz_seq_between_length. *)
+  (*     } *)
+  (*     iSplitL "Hmmap_old". *)
+  (*     + iApply (big_sepM_to_big_sepL2 with "Hmmap_old"). *)
+  (*       { apply NoDup_logical_region. } *)
+  (*       { by rewrite map_length finz_seq_between_length. } *)
+  (*     + iApply (big_sepM_to_big_sepL2 with "Hmmap_new"). *)
+  (*       { apply NoDup_logical_region. } *)
+  (*       { by rewrite map_length finz_seq_between_length. } *)
 
-    - (* Success false *)
-      iApply "Hφ"; iRight.
-      rewrite /incrementLPC in Hincr_PC; simplify_map_eq.
-      iExtractList "Hrmap" [PC; dst; src] as ["HPC"; "Hdst"; "Hsrc"].
-      iClear "Hrmap".
-      iFrame.
-      iDestruct (big_sepM_insert with "Hmmap") as "[Hpc_a Hmmap]".
-      { apply not_elem_of_list_to_map.
-        rewrite fst_zip; [|rewrite map_length finz_seq_between_length; lia].
-        intros Hcontra.
-        apply elem_of_list_fmap_2 in Hcontra.
-        destruct Hcontra as (? & Ha & ?); simplify_eq.
-      }
-      iFrame.
-      iApply (big_sepM_to_big_sepL2 with "Hmmap").
-      { apply NoDup_logical_region. }
-      { by rewrite map_length finz_seq_between_length. }
-  Qed.
+  (*   - (* Success false *) *)
+  (*     iApply "Hφ"; iRight. *)
+  (*     rewrite /incrementLPC in Hincr_PC; simplify_map_eq. *)
+  (*     iExtractList "Hrmap" [PC; dst; src] as ["HPC"; "Hdst"; "Hsrc"]. *)
+  (*     iClear "Hrmap". *)
+  (*     iFrame. *)
+  (*     iDestruct (big_sepM_insert with "Hmmap") as "[Hpc_a Hmmap]". *)
+  (*     { apply not_elem_of_list_to_map. *)
+  (*       rewrite fst_zip; [|rewrite map_length finz_seq_between_length; lia]. *)
+  (*       intros Hcontra. *)
+  (*       apply elem_of_list_fmap_2 in Hcontra. *)
+  (*       destruct Hcontra as (? & Ha & ?); simplify_eq. *)
+  (*     } *)
+  (*     iFrame. *)
+  (*     iApply (big_sepM_to_big_sepL2 with "Hmmap"). *)
+  (*     { apply NoDup_logical_region. } *)
+  (*     { by rewrite map_length finz_seq_between_length. } *)
+  (* Qed. *)
 
   (* TODO merge wp_opt from Dominique's branch and use it *)
   (* TODO small toy program example that uses is_unique *)
